Flex

src/Contracts/Flex/Functions/Funcs.v
@@ -37,6 +37,11 @@ Require Import TradingPair.ClassTypesNotations.
 Require Import TONTokenWallet.ClassTypesNotations.
 Require Import Wrapper.ClassTypesNotations.
 
+Inductive code_type :=
+trade_pair_code | xchg_pair_code | wrapper_code | ext_wallet_code | flex_wallet_code 
+| price_code | xchg_price_code | no_such_code.
+
+
 Unset Typeclasses Iterative Deepening.
 Set Typeclasses Depth 30.
 
@@ -64,128 +69,208 @@ Existing Instance LedgerPruvendoRecord.
 Definition constructor ( deployer_pubkey :  uint256 ) ( ownership_description : String ) ( owner_address :  optional address ) 
                        ( tons_cfg :  TonsConfigLRecord ) ( deals_limit :  uint8 ) ( listing_cfg :  ListingConfigLRecord ) 
                        : UExpression PhantomType true . 
- 	 	 refine {{ _deployer_pubkey_ := #{ deployer_pubkey } ; { _ } }} . 
- 	 	 refine {{ _ownership_description_ := #{ ownership_description } ; { _ } }} . 
- 	 	 refine {{ _owner_address_ := #{ owner_address } ; { _ } }} . 
- 	 	 refine {{ _deals_limit_ := #{ deals_limit } ; { _ } }} . 
- 	 	 refine {{ _tons_cfg_ := #{ tons_cfg } ; { _ } }} . 
- 	 	 refine {{ _listing_cfg_ := #{ listing_cfg } ; { _ } }} . 
- 	 	 refine {{ _workchain_id_ := (tvm_myaddr ()) ↑ address.workchain_id ; { _ } }} . 
- 	 	 refine {{ require_ ( (((#{listing_cfg}) ↑ ListingConfig.register_pair_cost) >= 
+ 	refine {{ _deployer_pubkey_ := #{ deployer_pubkey } ; { _ } }} . 
+ 	refine {{ _ownership_description_ := #{ ownership_description } ; { _ } }} . 
+ 	refine {{ _owner_address_ := #{ owner_address } ; { _ } }} . 
+ 	refine {{ _deals_limit_ := #{ deals_limit } ; { _ } }} . 
+ 	refine {{ _tons_cfg_ := #{ tons_cfg } ; { _ } }} . 
+ 	refine {{ _listing_cfg_ := #{ listing_cfg } ; { _ } }} . 
+ 	refine {{ _workchain_id_ := (tvm_myaddr ()) ↑ address.workchain_id ; { _ } }} . 
+ 	refine {{ require_ ( (((#{listing_cfg}) ↑ ListingConfig.register_pair_cost) >= 
        ( (#{listing_cfg}) ↑ ListingConfig.reject_pair_cost )
                           + ( (#{listing_cfg}) ↑ ListingConfig.register_return_value ) ) , error_code::costs_inconsistency ) ; { _ } }} . 
-refine {{ return_ {} }} .
-Defined . 
-
-Print constructor .
+  refine {{ return_ {} }} .
+Defined. 
 
 Definition constructor_left { R a1 a2 a3 a4 a5 a6 }  ( deployer_pubkey : URValue uint256 a1 ) 
-                                                      ( ownership_description : URValue ( String ) a2 ) 
-                                                      ( owner_address : URValue ( optional address ) a3 ) 
-                                                      ( tons_cfg : URValue ( TonsConfigLRecord ) a4 ) 
-                                                      ( deals_limit : URValue uint8 a5 ) 
-                                                      ( listing_cfg : URValue ListingConfigLRecord a6 ) 
-                                                      : UExpression R true := 
+                                                     ( ownership_description : URValue ( String ) a2 ) 
+                                                     ( owner_address : URValue ( optional address ) a3 ) 
+                                                     ( tons_cfg : URValue ( TonsConfigLRecord ) a4 ) 
+                                                     ( deals_limit : URValue uint8 a5 ) 
+                                                     ( listing_cfg : URValue ListingConfigLRecord a6 ) 
+                                                     : UExpression R true := 
  wrapULExpression (ursus_call_with_args (LedgerableWithArgs:= λ6 ) constructor deployer_pubkey ownership_description owner_address tons_cfg deals_limit listing_cfg ) . 
  
- Notation " 'constructor_' '(' deployer_pubkey ownership_description owner_address tons_cfg deals_limit listing_cfg ')' " := 
+Notation " 'constructor_' '(' deployer_pubkey ownership_description owner_address tons_cfg deals_limit listing_cfg ')' " := 
  ( constructor_left deployer_pubkey ownership_description owner_address tons_cfg deals_limit listing_cfg ) 
  (in custom ULValue at level 0 , deployer_pubkey custom URValue at level 0 , ownership_description custom URValue at level 0 , 
   owner_address custom URValue at level 0 , tons_cfg custom URValue at level 0 , deals_limit custom URValue at level 0 ,
   listing_cfg custom URValue at level 0 ) : ursus_scope . 
- 
-(*   void setSpecificCode(uint8 type, cell code) {
-    switch (static_cast<code_type>(type.get())) {
-    case code_type::trade_pair_code: setPairCode(code); return;
-    case code_type::xchg_pair_code: setXchgPairCode(code); return;
-    case code_type::wrapper_code: setWrapperCode(code); return;
-    case code_type::ext_wallet_code: setExtWalletCode(code); return;
-    case code_type::flex_wallet_code: setFlexWalletCode(code); return;
-    case code_type::price_code: setPriceCode(code); return;
-    case code_type::xchg_price_code: setXchgPriceCode(code); return;
-    }
-  }
- *)
 
-Definition setSpecificCode ( type :  uint8 ) ( code :  cell ) : UExpression PhantomType false .
-   (* refine {{ switch_ ( {} ) with { { _ } ;; { _ } ;; { _ } ;; { _ } ;; { _ } ;; { _ } ;; { _ } } ) }}.
-  refine {{ case_ trade_pair_code => setPairCode(code) ; return_ {} }}.
-  refine {{ case_ xchg_pair_code => setPairCode(code) ; return_ {} }}.
-  refine {{ case_ wrapper_code => setPairCode(code) ; return_ {} }}.
-  refine {{ case_ ext_wallet_code => setPairCode(code) ; return_ {} }}.
-  refine {{ case_ flex_wallet_code => setPairCode(code) ; return_ {} }}.
-  refine {{ case_ price_code => setPairCode(code) ; return_ {} }}.
-  refine {{ case_ xchg_price_code => setPairCode(code) ; return_ {} }}. *)
- 	 	 refine {{ return_ {} }} .
-Defined.
+Notation "code_type::trade_pair_code" := (sInject trade_pair_code) (in custom URValue at level 0) : ursus_scope.
+Notation "code_type::xchg_pair_code" := (sInject xchg_pair_code) (in custom URValue at level 0) : ursus_scope.
+Notation "code_type::wrapper_code" := (sInject wrapper_code) (in custom URValue at level 0) : ursus_scope.
+Notation "code_type::ext_wallet_code" := (sInject ext_wallet_code) (in custom URValue at level 0) : ursus_scope.
+Notation "code_type::flex_wallet_code" := (sInject flex_wallet_code) (in custom URValue at level 0) : ursus_scope.
+Notation "code_type::price_code" := (sInject price_code) (in custom URValue at level 0) : ursus_scope.
+Notation "code_type::xchg_price_code" := (sInject xchg_price_code) (in custom URValue at level 0) : ursus_scope.
+
+Instance code_type_equable: XBoolEquable boolean code_type  :=
+{ 
+  eqb := fun x y => match x,y with
+                    | trade_pair_code, trade_pair_code => xBoolTrue
+                    | xchg_pair_code, xchg_pair_code => xBoolTrue
+                    | wrapper_code, wrapper_code => xBoolTrue
+                    | ext_wallet_code, ext_wallet_code => xBoolTrue
+                    | flex_wallet_code, flex_wallet_code => xBoolTrue
+                    | price_code, price_code => xBoolTrue
+                    | xchg_price_code, xchg_price_code => xBoolTrue
+                    | _, _ => xBoolFalse
+                    end
+}.
+
+Instance code_type_integerable : Integerable N code_type :=
+{
+  toInteger := fun ct => match ct with
+                         | trade_pair_code => 0
+                         | xchg_pair_code => 1
+                         | wrapper_code => 2
+                         | ext_wallet_code => 3
+                         | flex_wallet_code => 4
+                         | price_code => 5
+                         | xchg_price_code => 6
+                         | no_such_code => 999
+                         end;
+  fromInteger := fun n => match n with
+                          | 0 => trade_pair_code
+                          | 1 => xchg_pair_code
+                          | 2 => wrapper_code
+                          | 3 => ext_wallet_code
+                          | 4 => flex_wallet_code
+                          | 5 => price_code
+                          | 6 => xchg_price_code
+                          | _ => no_such_code
+                          end }.
 
 Definition setPairCode ( code :  cell ) : UExpression PhantomType true . 
-  refine {{ require_ ( ( ~ _pair_code_ ) , error_code::cant_override_code ) ; { _ } }} . 
+  refine {{ require_ ( ~ _pair_code_ , error_code::cant_override_code ) ; { _ } }} . 
   refine {{ require_ ( ( msg_pubkey () == _deployer_pubkey_ ) ,  error_code::sender_is_not_deployer  ) ; { _ } }} . 
   refine {{ tvm_accept () ; { _ } }} .   
-(*   refine {{ require_ ( ( (#{code}) -> ctos () -> sref () == #{2} ) ,  error_code::unexpected_refs_count_in_code  ) ; { _ } }} . *)
-  refine {{ _pair_code_ := {} (* builder ( ) . stslice ( #{code} -> to_slice () ) . stref ( build ( Address { tvm_myaddr ( ) } ) . endc ( ) ) . endc ( ) *) ; {_} }} . 
- refine {{ return_ {} }}.
+  refine {{ require_ ( ( (#{code}) -> ctos () -> srefs () ) == #{2} ,  error_code::unexpected_refs_count_in_code  ) ; { _ } }} . 
+  refine {{ _pair_code_ := (builder() -> stslice ( #{code} -> ctos () ) -> stref ( build ( σ tvm_myaddr () ) -> endc ()) -> endc ()) -> set ()  ; {_} }} . 
+  refine {{ return_ {} }}.
 Defined . 
+
+Definition setPairCode_left { R a1 }  ( code : URValue cell a1 ) : UExpression R true := 
+ wrapULExpression (ursus_call_with_args (LedgerableWithArgs := λ1) setPairCode code ) . 
  
+Notation " 'setPairCode_' '(' code ')' " := 
+ ( setPairCode_left code ) 
+ (in custom ULValue at level 0 , code custom URValue at level 0 ) : ursus_scope . 
+
 Definition setXchgPairCode ( code :  cell ) : UExpression PhantomType true . 
-    refine {{ require_ ( ( ~ _xchg_pair_code_ ) , error_code::cant_override_code ) ; { _ } }} . 
-    refine {{ require_ ( ( msg_pubkey () == _deployer_pubkey_ ) , error_code::sender_is_not_deployer ) ; { _ } }} . 
+    refine {{ require_ ( ~ _xchg_pair_code_ , error_code::cant_override_code ) ; { _ } }} . 
+    refine {{ require_ ( msg_pubkey () == _deployer_pubkey_ , error_code::sender_is_not_deployer ) ; { _ } }} . 
     refine {{ tvm_accept () ; { _ } }} . 
-    (* refine {{ require_ ( ( (#{code}) -> to_slice () -> refs () == #{2} ) , error_code::unexpected_refs_count_in_code ) ; { _ } }} .  *)
-    refine {{ _xchg_pair_code_ := {}(* builder ( ) . stslice ( #{code} -> to_slice () ) . stref ( build ( Address { tvm_myaddr ( ) } ) . endc ( ) ) . endc ( ) *) ; {_} }} . 
+    refine {{ require_ ( (#{code}) -> ctos () -> srefs () == #{2}  , error_code::unexpected_refs_count_in_code ) ; { _ } }} .  
+    refine {{ _xchg_pair_code_ := ( builder() -> stslice (#{code} -> ctos ()) -> stref ( build ( σ tvm_myaddr () ) -> endc () ) -> endc () ) -> set () ; {_} }} . 
     refine {{ return_ {} }}.
 Defined . 
+
+Definition setXchgPairCode_left { R a1 }  ( code : URValue cell a1 ) : UExpression R true := 
+ wrapULExpression (ursus_call_with_args (LedgerableWithArgs := λ1) setXchgPairCode code ) . 
  
+Notation " 'setXchgPairCode_' '(' code ')' " := 
+ ( setXchgPairCode_left code ) 
+ (in custom ULValue at level 0 , code custom URValue at level 0 ) : ursus_scope . 
+
+
 Definition setWrapperCode ( code :  cell ) : UExpression PhantomType true . 
-    refine {{ require_ ( ( ! _wrapper_code_ ) , error_code::cant_override_code ) ; { _ } }} . 
-    refine {{ require_ ( ( msg_pubkey () == _deployer_pubkey_ ) , error_code::sender_is_not_deployer ) ; { _ } }} . 
+    refine {{ require_ ( ~ _wrapper_code_ , error_code::cant_override_code ) ; { _ } }} . 
+    refine {{ require_ ( msg_pubkey () == _deployer_pubkey_ , error_code::sender_is_not_deployer ) ; { _ } }} . 
     refine {{ tvm_accept () ; { _ } }} . 
-   (*  refine {{ require_ ( ( (#{code}) -> to_slice () -> refs () == #{2} ) , error_code::unexpected_refs_count_in_code ) ; { _ } }} .  *)
-    refine {{ _wrapper_code_ := {} (* builder ( ) . stslice ( #{code} -> to_slice () ) . stref ( build ( Address { tvm_myaddr ( ) } ) . endc ( ) ) . endc ( ) *) ; {_} }} . 
+    refine {{ require_ ( (#{code}) -> ctos () -> srefs () == #{2} , error_code::unexpected_refs_count_in_code ) ; { _ } }} .  
+    refine {{ _wrapper_code_ := ( builder() -> stslice (#{code} -> ctos ()) -> stref ( build ( σ tvm_myaddr () ) -> endc () ) -> endc () ) -> set () ; {_} }} . 
     refine {{ return_ {} }}.
 Defined . 
 
+Definition setWrapperCode_left { R a1 }  ( code : URValue cell a1 ) : UExpression R true := 
+ wrapULExpression (ursus_call_with_args (LedgerableWithArgs := λ1) setWrapperCode code ) . 
+ 
+Notation " 'setWrapperCode_' '(' code ')' " := 
+ ( setWrapperCode_left code ) 
+ (in custom ULValue at level 0 , code custom URValue at level 0 ) : ursus_scope . 
 
- Definition setPriceCode ( code :  cell ) : UExpression PhantomType true . 
- 	 	 refine {{ require_ ( ( ~ _price_code_ ) ,  error_code::cant_override_code  ) ; { _ } }} . 
- 	 	 refine {{ require_ ( ( msg_pubkey () == _deployer_pubkey_ ) ,  error_code::sender_is_not_deployer  ) ; { _ } }} . 
- 	 	 refine {{ tvm_accept () ; { _ } }} . 
- 	 	 refine {{ _price_code_ -> set ( (#{code}) ) ; {_} }} . 
+
+Definition setPriceCode ( code :  cell ) : UExpression PhantomType true . 
+  refine {{ require_ ( ~ _price_code_ ,  error_code::cant_override_code  ) ; { _ } }} . 
+  refine {{ require_ ( msg_pubkey () == _deployer_pubkey_ ,  error_code::sender_is_not_deployer  ) ; { _ } }} . 
+  refine {{ tvm_accept () ; { _ } }} . 
+  refine {{ _price_code_ -> set ( #{code} ) ; {_} }} . 
   refine {{ return_ {} }}. 
- Defined . 
+Defined . 
+
+Definition setPriceCode_left { R a1 }  ( code : URValue cell a1 ) : UExpression R true := 
+ wrapULExpression (ursus_call_with_args (LedgerableWithArgs := λ1) setPriceCode code ) . 
  
- Definition setXchgPriceCode ( code :  cell ) : UExpression PhantomType true . 
- 	 	 refine {{ require_ ( ( ~ _xchg_price_code_ ) ,  error_code::cant_override_code  ) ; { _ } }} . 
- 	 	 refine {{ require_ ( ( msg_pubkey () == _deployer_pubkey_ ) ,  error_code::sender_is_not_deployer  ) ; { _ } }} . 
- 	 	 refine {{ tvm_accept () ; { _ } }} . 
- 	 	 refine {{ _xchg_price_code_ -> set ((#{code})) ; {_} }} . 
-  refine {{ return_ {} }}. 
- Defined .  
+Notation " 'setPriceCode_' '(' code ')' " := 
+ ( setPriceCode_left code ) 
+ (in custom ULValue at level 0 , code custom URValue at level 0 ) : ursus_scope . 
  
- Definition setExtWalletCode ( code :  cell ) : UExpression PhantomType true . 
- 	 	 refine {{ require_ ( ( ~ _ext_wallet_code_ ) ,   error_code::cant_override_code  ) ; { _ } }} . 
- 	 	 refine {{ require_ ( ( msg_pubkey () == _deployer_pubkey_ ) ,  error_code::sender_is_not_deployer  ) ; { _ } }} . 
- 	 	 refine {{ tvm_accept () ; { _ } }} . 
- 	 	 refine {{ _ext_wallet_code_ -> set ( (#{code}) ) ; {_} }} . 
+Definition setXchgPriceCode ( code :  cell ) : UExpression PhantomType true . 
+  refine {{ require_ ( ~ _xchg_price_code_ ,  error_code::cant_override_code  ) ; { _ } }} . 
+  refine {{ require_ ( msg_pubkey () == _deployer_pubkey_ ,  error_code::sender_is_not_deployer  ) ; { _ } }} . 
+  refine {{ tvm_accept () ; { _ } }} . 
+  refine {{ _xchg_price_code_ -> set ( #{code} ) ; {_} }} . 
   refine {{ return_ {} }}. 
- Defined . 
+Defined .  
+
+Definition setXchgPriceCode_left { R a1 }  ( code : URValue cell a1 ) : UExpression R true := 
+ wrapULExpression (ursus_call_with_args (LedgerableWithArgs := λ1) setXchgPriceCode code ) . 
  
- Definition setFlexWalletCode ( code :  cell ) : UExpression PhantomType true . 
- 	 	 refine {{ require_ ( ( ~ _flex_wallet_code_ ) ,  error_code::cant_override_code  ) ; { _ } }} . 
- 	 	 refine {{ require_ ( ( msg_pubkey () == _deployer_pubkey_ ) ,   error_code::sender_is_not_deployer  ) ; { _ } }} . 
- 	 	 refine {{ tvm_accept () ; { _ } }} . 
- 	 	 refine {{ _flex_wallet_code_ -> set ( (#{code}) ) ; {_} }} . 
+Notation " 'setXchgPriceCode_' '(' code ')' " := 
+ ( setXchgPriceCode_left code ) 
+ (in custom ULValue at level 0 , code custom URValue at level 0 ) : ursus_scope . 
+
+Definition setExtWalletCode ( code :  cell ) : UExpression PhantomType true . 
+  refine {{ require_ (  ~ _ext_wallet_code_  ,   error_code::cant_override_code  ) ; { _ } }} . 
+  refine {{ require_ (  msg_pubkey () == _deployer_pubkey_  ,  error_code::sender_is_not_deployer  ) ; { _ } }} . 
+  refine {{ tvm_accept () ; { _ } }} . 
+  refine {{ _ext_wallet_code_ -> set ( (#{code}) ) ; {_} }} . 
   refine {{ return_ {} }}. 
- Defined . 
+Defined . 
+
+Definition setExtWalletCode_left { R a1 }  ( code : URValue cell a1 ) : UExpression R true := 
+ wrapULExpression (ursus_call_with_args (LedgerableWithArgs := λ1) setExtWalletCode code ) . 
+ 
+Notation " 'setExtWalletCode_' '(' code ')' " := 
+ ( setExtWalletCode_left code ) 
+ (in custom ULValue at level 0 , code custom URValue at level 0 ) : ursus_scope . 
+
+Definition setFlexWalletCode ( code :  cell ) : UExpression PhantomType true . 
+  refine {{ require_ (  ~ _flex_wallet_code_  ,  error_code::cant_override_code  ) ; { _ } }} . 
+  refine {{ require_ (  msg_pubkey () == _deployer_pubkey_  , error_code::sender_is_not_deployer  ) ; { _ } }} . 
+  refine {{ tvm_accept () ; { _ } }} . 
+  refine {{ _flex_wallet_code_ -> set ( (#{code}) ) ; {_} }} . 
+  refine {{ return_ {} }}. 
+Defined . 
+
+Definition setFlexWalletCode_left { R a1 }  ( code : URValue cell a1 ) : UExpression R true := 
+ wrapULExpression (ursus_call_with_args (LedgerableWithArgs := λ1) setFlexWalletCode code ) . 
+ 
+Notation " 'setFlexWalletCode_' '(' code ')' " := 
+ ( setFlexWalletCode_left code ) 
+ (in custom ULValue at level 0 , code custom URValue at level 0 ) : ursus_scope . 
+
+Definition setSpecificCode ( type :  uint8 ) ( code :  cell ) : UExpression PhantomType true .
+  refine {{ switch_ ( #{fromInteger type} ) with { 
+    case_ #{trade_pair_code} => setPairCode_ ( #{code} ) ; exit_ {} ;; 
+    case_ #{xchg_pair_code} => setXchgPairCode_ ( #{code} ) ; exit_ {} ;;
+    case_ #{wrapper_code} => setWrapperCode_ ( #{code} ) ; exit_ {} ;; 
+    case_ #{ext_wallet_code} => setExtWalletCode_ ( #{code} ) ; exit_ {} ;; 
+    case_ #{flex_wallet_code} => setFlexWalletCode_ ( #{code} ) ; exit_ {} ;; 
+    case_ #{price_code} => setPriceCode_ ( #{code} ) ; exit_ {} ;; 
+    case_ #{xchg_price_code} => setXchgPriceCode_ ( #{code} ) ; exit_ {} } ; {_} }}.
+  refine {{ return_ {} }}.
+Defined.
 
 Definition check_owner : UExpression PhantomType true . 
- 	 	 refine {{ new 'internal_ownership : boolean @ "internal_ownership" :=  ~~ ? _owner_address_ ; { _ } }} . 
-  	 refine {{ if ( #{Internal} ) then { { _: UExpression PhantomType true } } else { { _: UExpression PhantomType true } } ; { _ } }} . 
- 	 	   refine {{ require_ ( !{ internal_ownership } && ( int_sender () == ( _owner_address_ ->get_default () ) ) ,  error_code::sender_is_not_my_owner )  }} . 
- 	 	   refine {{ require_ ( ( ~ !{ internal_ownership } && ( msg_pubkey () == _deployer_pubkey_ ) ) ,  error_code::sender_is_not_my_owner )  }} . 
-     refine {{ return_ {} }} .
- Defined . 
+  refine {{ new 'internal_ownership : boolean @ "internal_ownership" :=  ~~ ? _owner_address_ ; { _ } }} . 
+  refine {{ { if Internal then _: UEt else _ } ; { _ } }} . 
+  refine {{ require_ ( !{ internal_ownership } && ( int_sender () ==  * _owner_address_  ) ,  error_code::sender_is_not_my_owner )  }} . 
+  refine {{ require_ ( ( ~ !{ internal_ownership } && ( msg_pubkey () == _deployer_pubkey_ ) ) ,  error_code::sender_is_not_my_owner )  }} . 
+  refine {{ return_ {} }} .
+Defined . 
 
 Definition check_owner_left { R }  : UExpression R true := 
  wrapULExpression (ursus_call_with_args (LedgerableWithArgs:= λ0 ) check_owner ) . 
@@ -193,48 +278,44 @@ Definition check_owner_left { R }  : UExpression R true :=
 Notation " 'check_owner_' '(' ')' " :=  ( check_owner_left ) (in custom ULValue at level 0 ) : ursus_scope . 
 
 Definition transfer ( tto : address ) ( tons :  uint128 ) : UExpression PhantomType true . 
-  	 refine {{ check_owner_ ( ) ; { _ } }} .
- 	 	 refine {{ tvm_accept () ; { _ } }} . 
- 	 	 refine {{ tvm_transfer ( #{tto} , #{tons}  , TRUE , DEFAULT_MSG_FLAGS ) ; {_} }} . 
-refine {{ return_ {} }} .
+  refine {{ check_owner_ ( ) ; { _ } }} .
+  refine {{ tvm_accept () ; { _ } }} . 
+  refine {{ tvm_transfer ( #{tto} , #{tons}  , TRUE , DEFAULT_MSG_FLAGS_ ) ; {_} }} . 
+  refine {{ return_ {} }} .
 Defined . 
 
-Definition prepare_trading_pair_state_init_and_addr 
-( pair_data :  TradingPairClassTypesModule.DTradingPairLRecord ) 
-( pair_code :  cell ) 
-: UExpression ( StateInitLRecord # uint256 )  false . 
- 	 	refine {{ new 'pair_data_cl : cell @ "pair_data_cl" := 
-                       prepare_persistent_data_ ( {} , #{pair_data} ) ; { _ } }} . 
- 	 	 refine {{ new 'pair_init : StateInitLRecord @ "pair_init" :=  
+Definition prepare_trading_pair_state_init_and_addr ( pair_data :  TradingPairClassTypesModule.DTradingPairLRecord ) 
+                                                    ( pair_code :  cell ) 
+                                                    : UExpression ( StateInitLRecord # uint256 )  false . 
+  refine {{ new 'pair_data_cl : cell @ "pair_data_cl" := prepare_persistent_data_ ( {} , #{pair_data} ) ; { _ } }} . 
+ 	refine {{ new 'pair_init : StateInitLRecord @ "pair_init" :=  
                  [$ {}  ⇒ {StateInit_ι_split_depth} ;
                     {}  ⇒ {StateInit_ι_special} ; 
            ( (#{pair_code}) -> set () ) ⇒ {StateInit_ι_code} ; 
            ( (!{pair_data_cl}) -> set () ) ⇒ {StateInit_ι_data} ; 
             {}  ⇒ {StateInit_ι_library} $] ; { _ } }} .
-
- 	 	 refine {{ new 'pair_init_cl : cell @ "pair_init_cl" := {} ; { _ } }} . 
- 	 	 refine {{ { pair_init_cl } := build ( σ (!{pair_init}) ) -> make_cell ()  ; { _ } }} . 
-	 	 refine {{ return_ [ !{ pair_init } , tvm_hash ( !{pair_init_cl} ) ] }} .
- Defined .  
+ 	refine {{ new 'pair_init_cl : cell @ "pair_init_cl" := {} ; { _ } }} . 
+ 	refine {{ { pair_init_cl } := build ( σ (!{pair_init}) ) -> make_cell ()  ; { _ } }} . 
+	refine {{ return_ [ !{ pair_init } , tvm_hash ( !{pair_init_cl} ) ] }} .
+Defined .  
  
- Definition prepare_trading_pair_state_init_and_addr_right { a1 a2 }  
+Definition prepare_trading_pair_state_init_and_addr_right { a1 a2 }  
                   ( pair_data : URValue TradingPairClassTypesModule.DTradingPairLRecord a1 )
-                  ( pair_code : URValue cell a2 ) : URValue ( StateInitLRecord * uint256 )  ( orb a2 a1 ) := 
+                  ( pair_code : URValue cell a2 ) : URValue ( StateInitLRecord # uint256 )  ( orb a2 a1 ) := 
  wrapURExpression (ursus_call_with_args (LedgerableWithArgs:= λ2 ) prepare_trading_pair_state_init_and_addr pair_data pair_code ) . 
  
 Notation " 'prepare_trading_pair_state_init_and_addr_' '(' pair_data ',' pair_code ')' " := 
                   ( prepare_trading_pair_state_init_and_addr_right pair_data pair_code ) 
  (in custom URValue at level 0 , pair_data custom URValue at level 0 , pair_code custom URValue at level 0 ) : ursus_scope . 
   
-Definition prepare_trading_pair ( flex : address ) 
-                                 ( tip3_root : address ) 
-                                 ( pair_code : cell ) : UExpression ( StateInitLRecord # uint256 )  false . 
- 	 	 refine {{ new 'pair_data : TradingPairClassTypesModule.DTradingPairLRecord  @ "pair_data" :=  
+Definition prepare_trading_pair ( flex : address ) ( tip3_root : address ) 
+                                ( pair_code : cell ) : UExpression ( StateInitLRecord # uint256 )  false . 
+  refine {{ new 'pair_data : TradingPairClassTypesModule.DTradingPairLRecord  @ "pair_data" :=  
                	 	 [$ tvm_myaddr () ⇒ { DTradingPair_ι_flex_addr_ } ; 
                       #{tip3_root} ⇒ { DTradingPair_ι_tip3_root_ } ; 
                       0 ⇒ { DTradingPair_ι_min_amount_ } ; 
                       [ #{0%Z}, 0 ]  ⇒ { DTradingPair_ι_notify_addr_  }  $] ; { _ } }} . 
- 	 	 refine {{ return_ ( prepare_trading_pair_state_init_and_addr_ ( !{ pair_data } , #{pair_code} ) ) }} . 
+  refine {{ return_ ( prepare_trading_pair_state_init_and_addr_ ( !{ pair_data } , #{pair_code} ) ) }} . 
 Defined .
  
 Definition prepare_trading_pair_right { a1 a2 a3 }  ( flex : URValue address a1 ) 
@@ -242,62 +323,57 @@ Definition prepare_trading_pair_right { a1 a2 a3 }  ( flex : URValue address a1 
                                                      ( pair_code : URValue cell a3 ) : URValue ( StateInitLRecord * uint256 )  ( orb ( orb a3 a2 ) a1 ) := 
  wrapURExpression (ursus_call_with_args (LedgerableWithArgs:= λ3 ) prepare_trading_pair flex tip3_root pair_code ) . 
  
- Notation " 'prepare_trading_pair_' '(' flex ',' tip3_root ',' pair_code ')' " := ( prepare_trading_pair_right flex tip3_root pair_code ) 
+Notation " 'prepare_trading_pair_' '(' flex ',' tip3_root ',' pair_code ')' " := ( prepare_trading_pair_right flex tip3_root pair_code ) 
  (in custom URValue at level 0 , flex custom URValue at level 0 , tip3_root custom URValue at level 0 , pair_code custom URValue at level 0 ) : ursus_scope . 
 
- Definition registerTradingPair ( pubkey :  uint256 ) 
+Definition registerTradingPair ( pubkey :  uint256 ) 
                                 ( tip3_root : address ) 
                                 ( min_amount :  uint128  ) 
                                 ( notify_addr : address ) : UExpression address true . 
- 	 	 refine {{ require_ ( ( int_value () > ( _listing_cfg_ ↑  ListingConfig.register_pair_cost) ) ,  error_code::not_enough_funds  ) ; { _ } }} . 
- 	 	 refine {{ require_ ( ( ~ (_trading_pair_listing_requests_ ->contains ( #{pubkey} )) ) ,  
+  refine {{ require_ ( ( int_value () > ( _listing_cfg_ ↑  ListingConfig.register_pair_cost) ) ,  error_code::not_enough_funds  ) ; { _ } }} . 
+  refine {{ require_ ( ( ~ (_trading_pair_listing_requests_ ->contains ( #{pubkey} )) ) ,  
                error_code::trading_pair_with_such_pubkey_already_requested  ) ; { _ } }} . 
  
-  	 refine {{ _trading_pair_listing_requests_ -> set_at 
+  refine {{ _trading_pair_listing_requests_ -> set_at 
                ( #{pubkey} ,  [ int_sender () , 
                                 int_value ()  - 
                                   _listing_cfg_ ↑  ListingConfig.register_return_value , 
                                 #{tip3_root} , 
                                 #{min_amount} , 
                                 #{notify_addr}  ] ) ; { _ } }} . 
-  	 	 refine {{ set_int_return_value ( _listing_cfg_ ↑ ListingConfig.register_return_value ) ; { _ } }} .  
-      refine {{ new ( 'state_init : StateInitLRecord , 'std_addr : uint256 ) @ ("state_init", "std_addr") :=
+  refine {{ set_int_return_value ( _listing_cfg_ ↑ ListingConfig.register_return_value ) ; { _ } }} .  
+  refine {{ new ( 'state_init : StateInitLRecord , 'std_addr : uint256 ) @ ("state_init", "std_addr") :=
                 prepare_trading_pair_ ( tvm_myaddr () , #{tip3_root} , _pair_code_ -> get () ) ; { _ } }} .
- 	 	 refine {{ return_ [ _workchain_id_ , !{std_addr} ]  }} . 
- Defined .
+  refine {{ return_ [ _workchain_id_ , !{std_addr} ]  }} . 
+Defined .
  
 Definition approveTradingPairImpl ( pubkey : uint256 )
                                   ( trading_pair_listing_requests : trading_pairs_map ) 
                                   ( pair_code : cell ) 
                                   ( workchain_id : int ) 
-                                  ( listing_cfg : ListingConfigLRecord ) : UExpression ( address * (trading_pairs_map ) ) true . 
- 	 	 refine {{ new 'opt_req_info : optional TradingPairListingRequestLRecord @ "opt_req_info" := 
-                (#{trading_pair_listing_requests}) -> extract ( #{pubkey} ) ; {_} }} .
+                                  ( listing_cfg : ListingConfigLRecord ) : UExpression ( address # (trading_pairs_map ) ) true . 
+  vararg trading_pair_listing_requests "trading_pair_listing_requests".
 
-  
- 	 	 refine {{ require_ ( !{opt_req_info}  ,  error_code::trading_pair_not_requested  ) ; { _ } }} . 
- 	 	 refine {{ new 'req_info : TradingPairListingRequestLRecord @ "req_info" := 
-                              (!{opt_req_info}) -> get () ; { _ } }} . 
- 	 	 refine {{ new ( 'state_init : StateInitLRecord, 'std_addr : uint256 ) @ ("state_init", "std_addr") := 
+  refine {{ new 'opt_req_info : optional TradingPairListingRequestLRecord @ "opt_req_info" := 
+                {trading_pair_listing_requests} -> extract ( #{pubkey} ) ; {_} }} .
+  refine {{ require_ ( ~~ !{opt_req_info}  ,  error_code::trading_pair_not_requested  ) ; { _ } }} . 
+  refine {{ new 'req_info : TradingPairListingRequestLRecord @ "req_info" := * !{opt_req_info} ; { _ } }} . 
+  refine {{ new ( 'state_init : StateInitLRecord, 'std_addr : uint256 ) @ ("state_init", "std_addr") := 
                  prepare_trading_pair_ ( tvm_myaddr () , !{req_info} ↑ TradingPairListingRequest.tip3_root , #{pair_code} ) ; { _ } }} . 
- 	 	 refine {{ new 'trade_pair : address @ "trade_pair" := 
-                               [ #{ workchain_id } , !{std_addr} ] ; { _ } }} . 
-refine ( let trade_pair_ptr := {{ ITradingPairPtr [[ !{trade_pair}  ]] }} in 
+  refine {{ new 'trade_pair : address @ "trade_pair" := [ #{ workchain_id } , !{std_addr} ] ; { _ } }} . 
+  refine ( let trade_pair_ptr := {{ ITradingPairPtr [[ !{trade_pair}  ]] }} in 
               {{ {trade_pair_ptr} with {} ⤳ TradingPair.deploy ( !{state_init} ) ; {_} }} ).  
-
-      refine ( let trade_pair_ptr := {{ ITradingPairPtr [[ !{trade_pair}  ]] }} in 
-        {{ {trade_pair_ptr} with [$ (#{listing_cfg}) ↑ ListingConfig.pair_deploy_value ⇒ { Messsage_ι_value } ;
-                                     DEFAULT_MSG_FLAGS ⇒ { Messsage_ι_flags }  $] 
+  refine {{ {trade_pair_ptr} with [$ (#{listing_cfg}) ↑ ListingConfig.pair_deploy_value ⇒ { Messsage_ι_value } ;
+                                     #{DEFAULT_MSG_FLAGS} ⇒ { Messsage_ι_flags }  $] 
                         ⤳ TradingPair.onDeploy (!{req_info} ↑ TradingPairListingRequest.min_amount , 
                                                 (#{listing_cfg}) ↑ ListingConfig.pair_keep_balance , 
-                                                !{req_info} ↑ TradingPairListingRequest.notify_addr ) ; { _ } }} ).
- 	 	 refine {{ new 'remaining_funds : uint128 @ "remaining_funds" :=   
- 	 	   !{req_info} ↑ TradingPairListingRequest.client_funds - 
+                                                !{req_info} ↑ TradingPairListingRequest.notify_addr ) ; { _ } }} .
+  refine {{ new 'remaining_funds : uint128 @ "remaining_funds" :=  
+            !{req_info} ↑ TradingPairListingRequest.client_funds - 
             (#{listing_cfg}) ↑ ListingConfig.register_pair_cost ; { _ } }} . 
-refine {{ IListingAnswerPtr [[  !{req_info} ↑ TradingPairListingRequest.client_addr ]]
+  refine {{ IListingAnswerPtr [[  !{req_info} ↑ TradingPairListingRequest.client_addr ]]
           with [$ !{remaining_funds} ⇒ { Messsage_ι_value } $]  ⤳ .onTradingPairApproved ( #{pubkey} , !{trade_pair} ) ; {_} }}. 
-
- 	 	 refine {{ return_ [ !{trade_pair} , #{trading_pair_listing_requests} ] }} . 
+  refine {{ return_ [ !{trade_pair} , !{trading_pair_listing_requests} ] }} . 
 Defined .
 
 Definition approveTradingPairImpl_right { a1 a2 a3 a4 a5 } ( pubkey : URValue uint256 a1 ) 
@@ -313,18 +389,18 @@ Notation " 'approveTradingPairImpl_' '(' pubkey , trading_pair_listing_requests 
  (in custom URValue at level 0 , pubkey custom URValue at level 0 , trading_pair_listing_requests custom URValue at level 0 , 
   pair_code custom URValue at level 0 , workchain_id custom URValue at level 0 , listing_cfg custom URValue at level 0 ) : ursus_scope . 
 
- Definition approveTradingPair ( pubkey :  uint256 ) : UExpression address true . 
-  	 refine {{ check_owner_ ( ) ; { _ } }} .
- 	 	 refine {{ tvm_accept () ; { _ } }} .
- 	 	 refine {{ new ( 'trade_pair : address , 'new_trading_pair_listing_requests : trading_pairs_map ) 
+Definition approveTradingPair ( pubkey :  uint256 ) : UExpression address true . 
+  refine {{ check_owner_ ( ) ; { _ } }} .
+  refine {{ tvm_accept () ; { _ } }} .
+  refine {{ new ( 'trade_pair : address , 'new_trading_pair_listing_requests : trading_pairs_map ) 
                     @ ("trade_pair", "new_trading_pair_listing_requests")  := 
             approveTradingPairImpl_ ( #{pubkey} , _trading_pair_listing_requests_ , _pair_code_ -> get () , _workchain_id_ , _listing_cfg_ ) ; { _ } }} . 
- 	 	 refine {{ _trading_pair_listing_requests_ := !{new_trading_pair_listing_requests} ; { _ } }} . 
- 	 	 refine {{ if ( #{Internal} ) then { { _ } } else { exit_ {} } ; { _ } }} . 
- 	 	 refine {{ new 'value_gr : uint @ "value_gr" := int_value ()  ; { _ } }} . 
-  	 	 refine {{ tvm_rawreserve ( tvm_balance () - !{value_gr} ,  rawreserve_flag::up_to  )  (* ; { _ } *) }} .
- 	 	 refine {{ set_int_return_flag ( #{SEND_ALL_GAS} ) ; {_} }} .
- 	 refine {{ return_ !{ trade_pair } }} . 
+  refine {{ _trading_pair_listing_requests_ := !{new_trading_pair_listing_requests} ; { _ } }} . 
+  refine {{ { if Internal then _ else {{ return_ {} }} } ; { _ } }} . 
+  refine {{ new 'value_gr : uint @ "value_gr" := int_value ()  ; { _ } }} . 
+  refine {{ tvm_rawreserve ( tvm_balance () - !{value_gr} ,  rawreserve_flag::up_to  ) ; {_} }} .
+  refine {{ set_int_return_flag ( #{SEND_ALL_GAS} ) }} .
+  refine {{ return_ !{ trade_pair } }} . 
 Defined .
  
 Definition approveTradingPair_right { a1 }  ( pubkey : URValue uint256 a1 ) : URValue address true := 
@@ -335,17 +411,18 @@ Notation " 'approveTradingPair_' '(' pubkey ')' " :=  ( approveTradingPair_right
 
 Definition rejectTradingPairImpl ( pubkey : uint256 ) 
                                  ( trading_pair_listing_requests : trading_pairs_map ) 
-                                 ( listing_cfg :  ListingConfigLRecord ) : UExpression (trading_pairs_map ) true . 
- 	 	 refine {{ new 'opt_req_info : optional TradingPairListingRequestLRecord @ "opt_req_info" := 
-                 (#{trading_pair_listing_requests}) -> extract ( #{pubkey} ) ; { _ } }} .  
- 	 	 refine {{ require_ ( !{ opt_req_info }  ,  error_code::trading_pair_not_requested  ) ; { _ } }} . 
- 	 	 refine {{ new 'req_info : ( TradingPairListingRequestLRecord ) @ "req_info" := 
-                    (!{opt_req_info}) -> get ()  ; { _ } }} . 
- 	 	 refine {{ new 'remaining_funds : uint128 @ "remaining_funds" := 
-            ( (!{req_info}) ↑ TradingPairListingRequest.client_funds ) - ( (#{listing_cfg}) ↑ ListingConfig.reject_pair_cost ) ; { _ } }} . 
-refine {{ IListingAnswerPtr [[  !{req_info} ↑ TradingPairListingRequest.client_addr ]]
-          with [$ !{remaining_funds} ⇒ { Messsage_ι_value } $]  ⤳ .onTradingPairRejected ( #{pubkey} ) ; {_} }}.                                                               
- 	 	 refine {{ return_ #{trading_pair_listing_requests} }} . 
+                                 ( listing_cfg :  ListingConfigLRecord ) : UExpression (trading_pairs_map ) true .
+  vararg trading_pair_listing_requests "trading_pair_listing_requests".                                
+  refine {{ new 'opt_req_info : optional TradingPairListingRequestLRecord @ "opt_req_info" := 
+                 {trading_pair_listing_requests} -> extract ( #{pubkey} ) ; { _ } }} .  
+  refine {{ require_ ( ~~!{ opt_req_info }  ,  error_code::trading_pair_not_requested  ) ; { _ } }} . 
+  refine {{ new 'req_info : ( TradingPairListingRequestLRecord ) @ "req_info" := *!{opt_req_info} ; { _ } }} . 
+  refine {{ new 'remaining_funds : uint128 @ "remaining_funds" := 
+            ( (!{req_info}) ↑ TradingPairListingRequest.client_funds ) - 
+            ( (#{listing_cfg}) ↑ ListingConfig.reject_pair_cost ) ; { _ } }} . 
+  refine {{ IListingAnswerPtr [[  !{req_info} ↑ TradingPairListingRequest.client_addr ]]
+          with [$ !{remaining_funds} ⇒ { Messsage_ι_value } $]  ⤳ .onTradingPairRejected ( #{pubkey} ) ; {_} }}.
+  refine {{ return_ !{trading_pair_listing_requests} }} . 
 Defined . 
 
 Definition rejectTradingPairImpl_right { a1 a2 a3 }  ( pubkey : URValue  uint256  a1 )
@@ -357,19 +434,19 @@ Definition rejectTradingPairImpl_right { a1 a2 a3 }  ( pubkey : URValue  uint256
  ( rejectTradingPairImpl_right pubkey trading_pair_listing_requests listing_cfg ) 
  (in custom URValue at level 0 , pubkey custom URValue at level 0 , trading_pair_listing_requests custom URValue at level 0 , listing_cfg custom URValue at level 0 ) : ursus_scope .
 
- Definition rejectTradingPair ( pubkey :  uint256 ) : UExpression XBool true . 
+ Definition rejectTradingPair ( pubkey :  uint256 ) : UExpression boolean true . 
   	refine {{ check_owner_ ( ) ; { _ } }} .
  	 	refine {{ _trading_pair_listing_requests_ := 
               rejectTradingPairImpl_ ( #{pubkey} , _trading_pair_listing_requests_ , _listing_cfg_ ) ; { _ } }} . 
  	 	refine {{ new 'value_gr : uint @ "value_gr" := int_value () ; { _ } }} . 
   	refine {{ tvm_rawreserve ( tvm_balance () - !{value_gr} , rawreserve_flag::up_to  ) ; { _ } }} .
- 	 	refine {{ if ( #{Internal} ) then { { _ } } else { return_ {} } ; { _ } }} . 
+ 	 	refine {{ { if Internal then _ else {{ return_ {} }} } ; { _ } }} . 
  	  refine {{ {value_gr} := int_value () ; { _ } }} .  	 	 	 
     refine {{ set_int_return_flag ( #{SEND_ALL_GAS} ) }} .
- 	 refine {{ return_ TRUE }} .
+ 	  refine {{ return_ TRUE }} .
 Defined . 
 
-Definition rejectTradingPair_right { a1 }  ( pubkey : URValue uint256 a1 ) : URValue XBool true := 
+Definition rejectTradingPair_right { a1 }  ( pubkey : URValue uint256 a1 ) : URValue boolean true := 
  wrapURExpression (ursus_call_with_args (LedgerableWithArgs:= λ1 ) rejectTradingPair pubkey ) . 
  
 Notation " 'rejectTradingPair_' '(' pubkey ')' " := ( rejectTradingPair_right pubkey ) 
@@ -385,8 +462,7 @@ Definition prepare_xchg_pair_state_init_and_addr ( pair_data :  XchgPairClassTyp
                #{pair_code} -> set () ⇒ { StateInit_ι_code } ;
                !{pair_data_cl} -> set () ⇒ { StateInit_ι_data } ;
                {} ⇒ { StateInit_ι_library } $] ; { _ } }} .
-  refine {{ new 'pair_init_cl : cell @ "pair_init_cl" := 
-                     build ( σ !{ pair_init } ) -> make_cell () ; { _ } }} . 
+  refine {{ new 'pair_init_cl : cell @ "pair_init_cl" := build ( σ !{ pair_init } ) -> make_cell () ; { _ } }} . 
   refine {{ return_ [ !{ pair_init } , tvm_hash ( !{pair_init_cl} )  ] }} .
 Defined .
 
@@ -401,134 +477,105 @@ Notation " 'prepare_xchg_pair_state_init_and_addr_' '(' pair_data , pair_code ')
 Definition approveXchgPairImpl ( pubkey :  uint256 ) ( xchg_pair_listing_requests :  xchg_pairs_map ) 
                                ( xchg_pair_code :  cell ) ( workchain_id :  int ) ( listing_cfg :  ListingConfigLRecord ) 
                                : UExpression ( address # xchg_pairs_map )  true . 
-
- 	 	 refine {{ new 'opt_req_info : ( optional XchgPairListingRequestLRecord ) @ "opt_req_info" := 
-                         (#{xchg_pair_listing_requests}) -> extract ( #{pubkey} ) ; { _ } }} . 
- 	 	 refine {{ require_ ( !{ opt_req_info }  ,  error_code::xchg_pair_not_requested  ) ; { _ } }} . 
- 	 	 refine {{ new 'req_info : ( XchgPairListingRequestLRecord ) @ "req_info" := 
-                          (!{opt_req_info}) -> get () ; { _ } }} . (* 43'' *)
- 	 	 refine {{ new 'pair_data : ( XchgPairClassTypesModule.DXchgPairLRecord ) @ "pair_data" :=  
+  vararg xchg_pair_listing_requests "xchg_pair_listing_requests".
+  refine {{ new 'opt_req_info : optional XchgPairListingRequestLRecord @ "opt_req_info" := 
+                         {xchg_pair_listing_requests} -> extract ( #{pubkey} ) ; { _ } }} . 
+  refine {{ require_ ( ~~!{ opt_req_info }  ,  error_code::xchg_pair_not_requested  ) ; { _ } }} . 
+  refine {{ new 'req_info :  XchgPairListingRequestLRecord  @ "req_info" := *!{opt_req_info} ; { _ } }} .
+  refine {{ new 'pair_data : XchgPairClassTypesModule.DXchgPairLRecord @ "pair_data" :=  
                	 	 [$ tvm_myaddr () ⇒ { DXchgPair_ι_flex_addr_ } ; 
                       !{req_info} ↑ XchgPairListingRequest.tip3_major_root ⇒ { DXchgPair_ι_tip3_major_root_ } ; 
                       !{req_info} ↑ XchgPairListingRequest.tip3_minor_root ⇒ { DXchgPair_ι_tip3_minor_root_ } ; 
                       0 ⇒ { DXchgPair_ι_min_amount_ } ; 
-                  [ #{0%Z} , 0 ] ⇒ { DXchgPair_ι_notify_addr_ } $] ; { _ } }} . (*45''*) 
-
- 	 	 refine {{ new ( 'state_init : StateInitLRecord , 'std_addr : uint256 ) @ ( "state_init" , "std_addr" ) := prepare_xchg_pair_state_init_and_addr_ ( !{pair_data} , #{xchg_pair_code} ) ; { _ } }} . 
-      refine {{ new 'xchg_pair : address @ "xchg_pair" := 
-                      [ #{workchain_id} , !{std_addr} ] ; { _ } }} .
-    refine ( let xchg_pair_ptr := {{ IXchgPairPtr [[ !{xchg_pair}  ]] }} in 
+                  [ #{0%Z} , 0 ] ⇒ { DXchgPair_ι_notify_addr_ } $] ; { _ } }} . 
+  refine {{ new ( 'state_init : StateInitLRecord , 'std_addr : uint256 ) 
+                   @ ( "state_init" , "std_addr" ) := prepare_xchg_pair_state_init_and_addr_ ( !{pair_data} , #{xchg_pair_code} ) ; { _ } }} . 
+  refine {{ new 'xchg_pair : address @ "xchg_pair" := [ #{workchain_id} , !{std_addr} ] ; { _ } }} .
+  refine ( let xchg_pair_ptr := {{ IXchgPairPtr [[ !{xchg_pair}  ]] }} in 
               {{ {xchg_pair_ptr} with {} ⤳ XchgPair.deploy ( !{state_init} ) ; {_} }} ).  
-
-      refine ( let xchg_pair_ptr := {{ IXchgPairPtr [[ !{xchg_pair}  ]] }} in 
-        {{ {xchg_pair_ptr} with [$ ((#{listing_cfg}) ↑ ListingConfig.pair_deploy_value) ⇒ { Messsage_ι_value } ;
+  refine {{ {xchg_pair_ptr} with [$ ((#{listing_cfg}) ↑ ListingConfig.pair_deploy_value) ⇒ { Messsage_ι_value } ;
                                     FALSE  ⇒ { Messsage_ι_bounce } ;
-                                    DEFAULT_MSG_FLAGS ⇒ { Messsage_ι_flags }  $] 
+                                    #{DEFAULT_MSG_FLAGS} ⇒ { Messsage_ι_flags }  $] 
                         ⤳ XchgPair.onDeploy (!{req_info} ↑ XchgPairListingRequest.min_amount , 
                                 (#{listing_cfg}) ↑ ListingConfig.pair_keep_balance , 
-                                !{req_info} ↑ XchgPairListingRequest.notify_addr ) ; { _ } }} ).
- 	 	 refine {{ new 'remaining_funds : uint128 @ "remaining_funds" := !{req_info} ↑ XchgPairListingRequest.client_funds - 
-                                                                     ( #{listing_cfg} ) ↑ ListingConfig.register_pair_cost  ; { _ } }} . 
-     refine {{ IListingAnswerPtr [[  !{req_info} ↑ XchgPairListingRequest.client_addr ]]
+                                !{req_info} ↑ XchgPairListingRequest.notify_addr ) ; { _ } }} .
+  refine {{ new 'remaining_funds : uint128 @ "remaining_funds" := !{req_info} ↑ XchgPairListingRequest.client_funds - 
+                                                                   ( #{listing_cfg} ) ↑ ListingConfig.register_pair_cost  ; { _ } }} . 
+  refine {{ IListingAnswerPtr [[  !{req_info} ↑ XchgPairListingRequest.client_addr ]]
           with [$ !{remaining_funds} ⇒ { Messsage_ι_value } $]  ⤳ .onXchgPairApproved ( #{pubkey} , !{xchg_pair} ) ; {_} }}.                                                               
- 	 	 refine {{ return_ [ !{xchg_pair} , #{xchg_pair_listing_requests} ] }} . 
- Defined .
+  refine {{ return_ [ !{xchg_pair} , !{xchg_pair_listing_requests} ] }} . 
+Defined .
  
- Definition approveXchgPairImpl_right { a1 a2 a3 a4 a5 }  
-( pubkey : URValue uint256 a1 ) 
-( xchg_pair_listing_requests : URValue xchg_pairs_map a2 ) 
-( xchg_pair_code : URValue cell a3 ) ( workchain_id : URValue int a4 ) 
-( listing_cfg : URValue ListingConfigLRecord a5 ) 
-: URValue ( address # xchg_pairs_map ) true := 
- wrapURExpression (ursus_call_with_args (LedgerableWithArgs:= λ5 ) approveXchgPairImpl 
- pubkey xchg_pair_listing_requests xchg_pair_code workchain_id listing_cfg ) . 
+Definition approveXchgPairImpl_right { a1 a2 a3 a4 a5 }  ( pubkey : URValue uint256 a1 ) 
+                                                         ( xchg_pair_listing_requests : URValue xchg_pairs_map a2 ) 
+                                                         ( xchg_pair_code : URValue cell a3 ) ( workchain_id : URValue int a4 ) 
+                                                         ( listing_cfg : URValue ListingConfigLRecord a5 ) 
+                                                         : URValue ( address # xchg_pairs_map ) true := 
+ wrapURExpression (ursus_call_with_args (LedgerableWithArgs:= λ5 ) approveXchgPairImpl pubkey xchg_pair_listing_requests xchg_pair_code workchain_id listing_cfg ) . 
  
- Notation " 'approveXchgPairImpl_' '(' pubkey , xchg_pair_listing_requests , xchg_pair_code , workchain_id , listing_cfg ')' " := 
- ( approveXchgPairImpl_right 
- pubkey xchg_pair_listing_requests xchg_pair_code workchain_id listing_cfg ) 
- (in custom URValue at level 0 , pubkey custom URValue at level 0 
- , xchg_pair_listing_requests custom URValue at level 0 
- , xchg_pair_code custom URValue at level 0 
- , workchain_id custom URValue at level 0 
- , listing_cfg custom URValue at level 0 ) : ursus_scope . 
+Notation " 'approveXchgPairImpl_' '(' pubkey , xchg_pair_listing_requests , xchg_pair_code , workchain_id , listing_cfg ')' " := 
+ ( approveXchgPairImpl_right pubkey xchg_pair_listing_requests xchg_pair_code workchain_id listing_cfg ) 
+ (in custom URValue at level 0 , pubkey custom URValue at level 0 , xchg_pair_listing_requests custom URValue at level 0 
+ , xchg_pair_code custom URValue at level 0 , workchain_id custom URValue at level 0 , listing_cfg custom URValue at level 0 ) : ursus_scope . 
 
- Definition rejectXchgPairImpl 
-( pubkey :  uint256 ) 
-( xchg_pair_listing_requests :  xchg_pairs_map ) 
-( listing_cfg :  ListingConfigLRecord ) : 
-UExpression xchg_pairs_map true . 
- 	 	 refine {{ new 'opt_req_info : ( optional XchgPairListingRequestLRecord ) @ "opt_req_info" := 
-                (#{xchg_pair_listing_requests}) -> extract (#{pubkey}) ; { _ } }} . 
- 	 	 refine {{ require_ ( !{ opt_req_info } ,  error_code::xchg_pair_not_requested  ) ; { _ } }} . 
- 	 	 refine {{ new 'req_info : ( XchgPairListingRequestLRecord ) @ "req_info" := 
-                  (!{opt_req_info}) -> get () ; { _ } }} . 
- 	 	 refine {{ new 'remaining_funds : uint128 @ "remaining_funds" := 
-          ( (!{req_info}) ↑ XchgPairListingRequest.client_funds )
-                 - ( (#{listing_cfg}) ↑ ListingConfig.reject_pair_cost ) ; { _ } }} . 
-refine {{ IListingAnswerPtr [[  !{req_info} ↑ XchgPairListingRequest.client_addr ]]
+Definition rejectXchgPairImpl ( pubkey :  uint256 ) ( xchg_pair_listing_requests :  xchg_pairs_map ) 
+                              ( listing_cfg :  ListingConfigLRecord ) :  UExpression xchg_pairs_map true . 
+  vararg xchg_pair_listing_requests "xchg_pair_listing_requests".                               
+  refine {{ new 'opt_req_info : optional XchgPairListingRequestLRecord @ "opt_req_info" := 
+                {xchg_pair_listing_requests} -> extract (#{pubkey}) ; { _ } }} . 
+  refine {{ require_ ( ~~!{ opt_req_info } ,  error_code::xchg_pair_not_requested  ) ; { _ } }} . 
+  refine {{ new 'req_info : ( XchgPairListingRequestLRecord ) @ "req_info" := *!{opt_req_info} ; { _ } }} . 
+  refine {{ new 'remaining_funds : uint128 @ "remaining_funds" := 
+          ( (!{req_info}) ↑ XchgPairListingRequest.client_funds ) -
+            ( (#{listing_cfg}) ↑ ListingConfig.reject_pair_cost ) ; { _ } }} . 
+  refine {{ IListingAnswerPtr [[  !{req_info} ↑ XchgPairListingRequest.client_addr ]]
           with [$ !{remaining_funds} ⇒ { Messsage_ι_value } $]  ⤳ .onXchgPairRejected ( #{pubkey} ) ; {_} }}.  
- 	 	 refine {{ return_ #{xchg_pair_listing_requests} }} . 
- Defined . 
+  refine {{ return_ !{xchg_pair_listing_requests} }} . 
+Defined . 
  
- Definition rejectXchgPairImpl_right { a1 a2 a3 } 
- ( pubkey : URValue uint256 a1 ) 
-( xchg_pair_listing_requests : URValue xchg_pairs_map a2 ) 
-( listing_cfg : URValue ListingConfigLRecord a3 ) 
-: URValue xchg_pairs_map true := 
- wrapURExpression (ursus_call_with_args (LedgerableWithArgs:= λ3 ) rejectXchgPairImpl 
- pubkey xchg_pair_listing_requests listing_cfg ) . 
+ Definition rejectXchgPairImpl_right { a1 a2 a3 } ( pubkey : URValue uint256 a1 ) 
+                                                  ( xchg_pair_listing_requests : URValue xchg_pairs_map a2 ) 
+                                                  ( listing_cfg : URValue ListingConfigLRecord a3 ) 
+                                                  : URValue xchg_pairs_map true := 
+ wrapURExpression (ursus_call_with_args (LedgerableWithArgs:= λ3 ) rejectXchgPairImpl pubkey xchg_pair_listing_requests listing_cfg ) . 
  
- Notation " 'rejectXchgPairImpl_' '(' pubkey , xchg_pair_listing_requests , listing_cfg ')' " := 
- ( rejectXchgPairImpl_right 
- pubkey xchg_pair_listing_requests listing_cfg ) 
- (in custom URValue at level 0 , pubkey custom URValue at level 0 
- , xchg_pair_listing_requests custom URValue at level 0 
- , listing_cfg custom URValue at level 0 ) : ursus_scope .
+Notation " 'rejectXchgPairImpl_' '(' pubkey , xchg_pair_listing_requests , listing_cfg ')' " := 
+ ( rejectXchgPairImpl_right pubkey xchg_pair_listing_requests listing_cfg ) 
+ (in custom URValue at level 0 , pubkey custom URValue at level 0 , 
+ xchg_pair_listing_requests custom URValue at level 0 , listing_cfg custom URValue at level 0 ) : ursus_scope .
 
- Definition prepare_wrapper_state_init_and_addr 
-( wrapper_code :  cell ) 
-( wrapper_data :  ( WrapperClassTypesModule.DWrapperLRecord ) ) 
-: UExpression ( StateInitLRecord * uint256 )  false . 
- 	 	 refine {{ new 'wrapper_data_cl : cell @ "wrapper_data_cl" :=  
-             prepare_persistent_data_ ( {} (* wrapper_replay_protection_t::init () *) , #{wrapper_data} ) ; { _ } }} . 
- 	 	 refine {{ new 'wrapper_init : StateInitLRecord @ "wrapper_init" := 
-
+Definition prepare_wrapper_state_init_and_addr ( wrapper_code :  cell ) ( wrapper_data : WrapperClassTypesModule.DWrapperLRecord ) 
+                                               : UExpression ( StateInitLRecord * uint256 )  false . 
+  refine {{ new 'wrapper_data_cl : cell @ "wrapper_data_cl" :=  
+            prepare_persistent_data_ ( wrapper_replay_protection_t::init ()  , #{wrapper_data} ) ; { _ } }} . 
+  refine {{ new 'wrapper_init : StateInitLRecord @ "wrapper_init" := 
                [$ {} ⇒ { StateInit_ι_split_depth } ; 
                   {} ⇒ { StateInit_ι_special } ;
                (#{wrapper_code}) -> set () ⇒ { StateInit_ι_code } ;
                (!{wrapper_data_cl}) -> set () ⇒ { StateInit_ι_data } ;  
                   {} ⇒ { StateInit_ι_library } 
                $]; { _ } }} . 
+  refine {{ new 'wrapper_init_cl : cell @ "wrapper_init_cl" := build ( σ !{ wrapper_init } ) -> make_cell () ; { _ } }} . 
+  refine {{ return_ [ !{ wrapper_init } ,  tvm_hash ( !{wrapper_init_cl} ) ] }} . 
+Defined . 
 
- 	 	 refine {{ new 'wrapper_init_cl : cell @ "wrapper_init_cl" := 
-                   build ( σ !{ wrapper_init } ) -> make_cell () ; { _ } }} . 
- 	 	 refine {{ return_ [ !{ wrapper_init } ,  tvm_hash ( !{wrapper_init_cl} ) ] }} . 
- Defined . 
-
- Definition prepare_wrapper_state_init_and_addr_right { a1 a2 }  ( wrapper_code : URValue cell a1 )
- ( wrapper_data : URValue ( WrapperClassTypesModule.DWrapperLRecord ) a2 ) : URValue ( StateInitLRecord * uint256 )  ( orb a2 a1 ) := 
- wrapURExpression (ursus_call_with_args (LedgerableWithArgs:= λ2 ) prepare_wrapper_state_init_and_addr 
- wrapper_code wrapper_data ) . 
+Definition prepare_wrapper_state_init_and_addr_right { a1 a2 }  ( wrapper_code : URValue cell a1 ) 
+                                                                ( wrapper_data : URValue WrapperClassTypesModule.DWrapperLRecord a2 ) 
+                                                                : URValue ( StateInitLRecord * uint256 )  ( orb a2 a1 ) := 
+ wrapURExpression (ursus_call_with_args (LedgerableWithArgs:= λ2 ) prepare_wrapper_state_init_and_addr wrapper_code wrapper_data ) . 
  
- Notation " 'prepare_wrapper_state_init_and_addr_' '(' wrapper_code , wrapper_data ')' " := 
- ( prepare_wrapper_state_init_and_addr_right 
- wrapper_code wrapper_data ) 
+Notation " 'prepare_wrapper_state_init_and_addr_' '(' wrapper_code , wrapper_data ')' " := 
+ ( prepare_wrapper_state_init_and_addr_right wrapper_code wrapper_data ) 
  (in custom URValue at level 0 , wrapper_code custom URValue at level 0 
  , wrapper_data custom URValue at level 0 ) : ursus_scope . 
 
- Definition prepare_external_wallet_state_init_and_addr 
-( name :  ( XString ) ) 
-( symbol :  ( XString ) ) 
-( decimals :  uint8 ) 
-( root_public_key :  uint256 ) 
-( wallet_public_key :  uint256 ) 
-( root_address : address ) 
-( owner_address :  ( optional address ) ) 
-( code :  cell ) 
-( workchain_id :  int ) 
-: UExpression ( StateInitLRecord # uint256 )  false .
+Definition prepare_external_wallet_state_init_and_addr ( name :  String ) ( symbol :  String ) 
+                                                       ( decimals :  uint8 ) ( root_public_key :  uint256 ) 
+                                                       ( wallet_public_key :  uint256 ) ( root_address : address ) 
+                                                       ( owner_address : optional address ) ( code :  cell ) 
+                                                       ( workchain_id :  int ) : UExpression ( StateInitLRecord # uint256 )  false .
 
-refine {{ new 'wallet_data : ( TONTokenWalletClassTypesModule.DTONTokenWalletExternalLRecord ) @ "wallet_data" := 
+  refine {{ new 'wallet_data : ( TONTokenWalletClassTypesModule.DTONTokenWalletExternalLRecord ) @ "wallet_data" := 
                  [$ 
                        (#{name}) ⇒ {DTONTokenWalletExternal_ι_name_ } ; 
                        (#{symbol}) ⇒ {DTONTokenWalletExternal_ι_symbol_ } ;
@@ -542,257 +589,214 @@ refine {{ new 'wallet_data : ( TONTokenWalletClassTypesModule.DTONTokenWalletExt
                        {} ⇒ {DTONTokenWalletExternal_ι_allowance_ } ; 
                        (#{workchain_id}) ⇒ {DTONTokenWalletExternal_ι_workchain_id_ } 
                                $] ; { _ } }} . 
-
- refine {{ new 'wallet_data_cl : cell @ "wallet_data_cl" :=
-             prepare_persistent_data_ ( {} (* external_wallet_replay_protection_t::init () *) , !{wallet_data} ) ; { _ } }} . 
- refine {{ new 'wallet_init : StateInitLRecord @ "wallet_init" := 
+  refine {{ new 'wallet_data_cl : cell @ "wallet_data_cl" := prepare_persistent_data_ ( external_wallet_replay_protection_t::init ()  , !{wallet_data} ) ; { _ } }} . 
+  refine {{ new 'wallet_init : StateInitLRecord @ "wallet_init" := 
                [$ {} ⇒ { StateInit_ι_split_depth } ; 
                   {} ⇒ { StateInit_ι_special } ;
                (#{code}) -> set () ⇒ { StateInit_ι_code } ;
                (!{wallet_data_cl}) -> set () ⇒ { StateInit_ι_data } ;  
                   {} ⇒ { StateInit_ι_library } 
                $]; { _ } }} . 
+  refine {{ new 'wallet_init_cl : cell @ "wallet_init_cl" := build ( σ !{ wallet_init } ) -> make_cell () ; { _ } }} . 
+  refine {{ return_ [ !{ wallet_init } ,  tvm_hash ( !{wallet_init_cl} )  ] }} . 
+Defined . 
 
- refine {{ new 'wallet_init_cl : cell @ "wallet_init_cl" := 
-                  build ( σ !{ wallet_init } ) -> make_cell () ; { _ } }} . 
- refine {{ return_ [ !{ wallet_init } ,  tvm_hash ( !{wallet_init_cl} )  ] }} . 
- Defined . 
-
- Definition prepare_external_wallet_state_init_and_addr_right { a1 a2 a3 a4 a5 a6 a7 a8 a9 }  
-( name : URValue ( XString ) a1 ) 
-( symbol :URValue  ( XString ) a2 ) 
-( decimals : URValue uint8 a3 )
- ( root_public_key : URValue uint256 a4 ) 
-( wallet_public_key : URValue uint256 a5 ) 
-( root_address : URValue address a6 ) 
-( owner_address : URValue ( optional address ) a7 )
- ( code : URValue cell a8 ) 
-( workchain_id : URValue int a9 ) 
-: URValue ( StateInitLRecord * uint256 )  ( orb ( orb ( orb ( orb ( orb ( orb ( orb ( orb a9 a8 ) a7 ) a6 ) a5 ) a4 ) a3 ) a2 ) a1 ) := 
- wrapURExpression (ursus_call_with_args (LedgerableWithArgs:= λ9 ) prepare_external_wallet_state_init_and_addr 
- name symbol decimals root_public_key wallet_public_key root_address owner_address code workchain_id ) . 
+Definition prepare_external_wallet_state_init_and_addr_right { a1 a2 a3 a4 a5 a6 a7 a8 a9 }  
+                                                              ( name : URValue String a1 ) 
+                                                              ( symbol :URValue  String a2 ) 
+                                                              ( decimals : URValue uint8 a3 )
+                                                              ( root_public_key : URValue uint256 a4 ) 
+                                                              ( wallet_public_key : URValue uint256 a5 ) 
+                                                              ( root_address : URValue address a6 ) 
+                                                              ( owner_address : URValue ( optional address ) a7 )
+                                                              ( code : URValue cell a8 ) 
+                                                              ( workchain_id : URValue int a9 ) 
+          : URValue ( StateInitLRecord * uint256 )  ( orb ( orb ( orb ( orb ( orb ( orb ( orb ( orb a9 a8 ) a7 ) a6 ) a5 ) a4 ) a3 ) a2 ) a1 ) := 
+ wrapURExpression (ursus_call_with_args (LedgerableWithArgs:= λ9 ) prepare_external_wallet_state_init_and_addr name symbol decimals root_public_key wallet_public_key root_address owner_address code workchain_id ) . 
  
- Notation " 'prepare_external_wallet_state_init_and_addr_' '(' name , symbol , decimals , root_public_key , wallet_public_key , root_address , owner_address , code , workchain_id ')' " := 
- ( prepare_external_wallet_state_init_and_addr_right 
- name symbol decimals root_public_key wallet_public_key root_address owner_address code workchain_id ) 
- (in custom URValue at level 0 , name custom URValue at level 0 
- , symbol custom URValue at level 0 
- , decimals custom URValue at level 0 
- , root_public_key custom URValue at level 0 
- , wallet_public_key custom URValue at level 0 
- , root_address custom URValue at level 0 
- , owner_address custom URValue at level 0 
- , code custom URValue at level 0 
+Notation " 'prepare_external_wallet_state_init_and_addr_' '(' name , symbol , decimals , root_public_key , wallet_public_key , root_address , owner_address , code , workchain_id ')' " := 
+ ( prepare_external_wallet_state_init_and_addr_right name symbol decimals root_public_key wallet_public_key root_address owner_address code workchain_id ) 
+ (in custom URValue at level 0 , name custom URValue at level 0 , symbol custom URValue at level 0 
+ , decimals custom URValue at level 0 , root_public_key custom URValue at level 0 , wallet_public_key custom URValue at level 0 
+ , root_address custom URValue at level 0 , owner_address custom URValue at level 0 , code custom URValue at level 0 
  , workchain_id custom URValue at level 0 ) : ursus_scope . 
 
- Definition approveWrapperImpl 
-( pubkey :  uint256 ) 
-( wrapper_listing_requests :  ( wrappers_map ) ) 
-( wrapper_code :  cell ) 
-( ext_wallet_code :  cell ) 
-( flex_wallet_code :  cell ) 
-( workchain_id :  int ) 
-( listing_cfg :  ListingConfigLRecord ) 
-: UExpression ( address # ( wrappers_map ) )  true . 
-
- refine {{ new 'opt_req_info : ( optional WrapperListingRequestLRecord ) @ "opt_req_info" := 
-             (#{wrapper_listing_requests}) -> extract ( #{pubkey} ) ; { _ } }} . 
- refine {{ require_ ( !{ opt_req_info }  ,  error_code::wrapper_not_requested  ) ; { _ } }} . 
- refine {{ new 'req_info : ( WrapperListingRequestLRecord ) @ "req_info" := 
-               (!{opt_req_info}) -> get () ; { _ } }} . 
- refine {{ new 'tip3cfg : ( Tip3ConfigLRecord ) @ "tip3cfg" := 
-                 (!{req_info}) ↑ WrapperListingRequest.tip3cfg ; { _ } }} .
- refine {{ new 'wrapper_data : ( WrapperClassTypesModule.DWrapperLRecord ) @ "wrapper_data" :=  
-               	 [$ ( (!{ tip3cfg }) ↑ Tip3Config.name ) ⇒ { DWrapper_ι_name_ } ; 
-               ( (!{ tip3cfg }) ↑ Tip3Config.symbol ) ⇒ { DWrapper_ι_symbol_ } ; 
-               ( (!{ tip3cfg }) ↑ Tip3Config.decimals ) ⇒ { DWrapper_ι_decimals_ } ; 
-               (#{workchain_id}) ⇒ { DWrapper_ι_workchain_id_ } ; 
-               (#{pubkey}) ⇒ { DWrapper_ι_root_public_key_ } ; 
-               {} ⇒ { DWrapper_ι_total_granted_ } ; 
-               {} ⇒ { DWrapper_ι_internal_wallet_code_ } ; 
-              ( ( tvm_myaddr () ) -> set () )  ⇒ { DWrapper_ι_owner_address_ } ; 
-               ( (#{listing_cfg}) ↑ ListingConfig.wrapper_keep_balance ) ⇒ { DWrapper_ι_start_balance_ } ; 
-               {} ⇒ { DWrapper_ι_external_wallet_ }  
-               $] ; { _ } }} . 
- 	 	 refine {{ new ( 'wrapper_init : StateInitLRecord , 
-                     'wrapper_hash_addr : uint256 ) @ ( "wrapper_init" , "wrapper_hash_addr" ) := 
+Definition approveWrapperImpl ( pubkey :  uint256 ) ( wrapper_listing_requests :  wrappers_map ) 
+                              ( wrapper_code :  cell ) ( ext_wallet_code :  cell ) 
+                              ( flex_wallet_code :  cell ) ( workchain_id :  int ) 
+                              ( listing_cfg :  ListingConfigLRecord ) : UExpression ( address # ( wrappers_map ) )  true . 
+  vararg wrapper_listing_requests "wrapper_listing_requests".
+ 
+  refine {{ new 'opt_req_info : ( optional WrapperListingRequestLRecord ) @ "opt_req_info" := 
+                {wrapper_listing_requests} -> extract ( #{pubkey} ) ; { _ } }} . 
+  refine {{ require_ ( !{ opt_req_info } ,  error_code::wrapper_not_requested  ) ; { _ } }} . 
+  refine {{ new 'req_info : ( WrapperListingRequestLRecord ) @ "req_info" := *!{opt_req_info} ; { _ } }} . 
+  refine {{ new 'tip3cfg : ( Tip3ConfigLRecord ) @ "tip3cfg" := !{req_info} ↑ WrapperListingRequest.tip3cfg ; { _ } }} .
+  refine {{ new 'wrapper_data : ( WrapperClassTypesModule.DWrapperLRecord ) @ "wrapper_data" :=  
+               	 [$ !{ tip3cfg } ↑ Tip3Config.name ⇒ { DWrapper_ι_name_ } ; 
+                    !{ tip3cfg } ↑ Tip3Config.symbol ⇒ { DWrapper_ι_symbol_ } ; 
+                    !{ tip3cfg } ↑ Tip3Config.decimals ⇒ { DWrapper_ι_decimals_ } ; 
+                    (#{workchain_id}) ⇒ { DWrapper_ι_workchain_id_ } ; 
+                    (#{pubkey}) ⇒ { DWrapper_ι_root_public_key_ } ; 
+                    {} ⇒ { DWrapper_ι_total_granted_ } ; 
+                    {} ⇒ { DWrapper_ι_internal_wallet_code_ } ; 
+                    tvm_myaddr () -> set () ⇒ { DWrapper_ι_owner_address_ } ; 
+                    (#{listing_cfg}) ↑ ListingConfig.wrapper_keep_balance  ⇒ { DWrapper_ι_start_balance_ } ; 
+                    {} ⇒ { DWrapper_ι_external_wallet_ }  $] ; { _ } }} . 
+  refine {{ new ( 'wrapper_init : StateInitLRecord , 'wrapper_hash_addr : uint256 ) 
+                @ ( "wrapper_init" , "wrapper_hash_addr" ) := 
                prepare_wrapper_state_init_and_addr_ ( #{wrapper_code} , !{wrapper_data} ) ; { _ } }} . 
- refine {{ new 'wrapper_addr : address @ "wrapper_addr" := 
-                            [ #{workchain_id} , !{wrapper_hash_addr} ]  ; { _ } }} .
- 	 	 refine {{ new ( 'wallet_init : StateInitLRecord , 'wallet_hash_addr : uint256 ) @ ( "wallet_init" , "wallet_hash_addr" ) := 
-       prepare_external_wallet_state_init_and_addr_ 
-           ( (!{ tip3cfg }) ↑ Tip3Config.name , 
-             (!{ tip3cfg }) ↑ Tip3Config.symbol , 
-             (!{ tip3cfg }) ↑ Tip3Config.decimals , 
-             (!{ tip3cfg }) ↑ Tip3Config.root_public_key , 
-             #{pubkey} , 
-             (!{ tip3cfg }) ↑ Tip3Config.root_address , 
-             (!{wrapper_addr}) -> set () , 
-              #{ext_wallet_code} , 
-              #{workchain_id} ) ; { _ } }} . 
- refine {{ new 'wallet_addr : address @ "wallet_addr" := {} ; { _ } }} .
-
-          
-refine ( let wallet_addr_ptr := {{ ITONTokenWalletPtr [[ !{wallet_addr}  ]] }} in 
+  refine {{ new 'wrapper_addr : address @ "wrapper_addr" := [ #{workchain_id} , !{wrapper_hash_addr} ]  ; { _ } }} .
+  refine {{ new ( 'wallet_init : StateInitLRecord , 'wallet_hash_addr : uint256 ) 
+              @ ( "wallet_init" , "wallet_hash_addr" ) := 
+              prepare_external_wallet_state_init_and_addr_ ( !{ tip3cfg } ↑ Tip3Config.name , 
+                                                             !{ tip3cfg } ↑ Tip3Config.symbol , 
+                                                             !{ tip3cfg } ↑ Tip3Config.decimals , 
+                                                             !{ tip3cfg } ↑ Tip3Config.root_public_key , 
+                                                             #{pubkey} , 
+                                                             !{ tip3cfg } ↑ Tip3Config.root_address , 
+                                                             !{wrapper_addr} -> set () , 
+                                                             #{ext_wallet_code} , 
+                                                             #{workchain_id} ) ; { _ } }} . 
+  refine {{ new 'wallet_addr : address @ "wrapper_addr" := [ #{workchain_id}, !{wallet_hash_addr} ] ; { _ } }} .
+  refine ( let wallet_addr_ptr := {{ ITONTokenWalletPtr [[ !{wallet_addr}  ]] }} in 
               {{ {wallet_addr_ptr} with [$ (#{listing_cfg}) ↑ ListingConfig.ext_wallet_balance ⇒ { Messsage_ι_value }  $] 
                                          ⤳ TONTokenWallet.deploy_noop ( !{wallet_init} ) ; {_} }} ).  
-refine ( let wallet_addr_ptr := {{ IWrapperPtr [[ !{wallet_addr}  ]] }} in 
-              {{ {wallet_addr_ptr} with [$ ((#{listing_cfg}) ↑ ListingConfig.wrapper_deploy_value) ⇒ { Messsage_ι_value }  $] 
-                                         ⤳ Wrapper.deploy ( !{wrapper_init} ) ; {_} }} ). (* Тут должен быть init, который делаент непонятно что *)  
-
- 	 	 refine {{ return_ [ !{wrapper_addr} , #{wrapper_listing_requests} ] }} . 
- Defined .
+  refine ( let wrapper_addr_ptr := {{ IWrapperPtr [[ !{wrapper_addr}  ]] }} in 
+              {{ {wrapper_addr_ptr} with [$ ((#{listing_cfg}) ↑ ListingConfig.wrapper_deploy_value) ⇒ { Messsage_ι_value }  $] 
+                                         ⤳ Wrapper.deploy ( !{wrapper_init} ) ; {_} }} ).
+  refine  {{ {wrapper_addr_ptr} with [$ ((#{listing_cfg}) ↑ ListingConfig.wrapper_deploy_value) ⇒ { Messsage_ι_value }  $] 
+                                         ⤳ .init ( !{wallet_addr} ) ; {_} }} .                                                                                   
+  refine {{ return_ [ !{wrapper_addr} , !{wrapper_listing_requests} ] }} . 
+Defined .
  
- Definition approveWrapperImpl_right { a1 a2 a3 a4 a5 a6 a7 }  
-( pubkey : URValue uint256 a1 ) 
-( wrapper_listing_requests : URValue (wrappers_map ) a2 )
-( wrapper_code : URValue cell a3 ) 
-( ext_wallet_code : URValue cell a4 ) 
-( flex_wallet_code : URValue cell a5 )
- ( workchain_id : URValue int a6 ) 
-( listing_cfg : URValue ListingConfigLRecord a7 ) 
-: URValue ( address # (wrappers_map ) )  true := 
- wrapURExpression (ursus_call_with_args (LedgerableWithArgs:= λ7 ) approveWrapperImpl 
- pubkey wrapper_listing_requests wrapper_code ext_wallet_code flex_wallet_code workchain_id listing_cfg ) . 
+ Definition approveWrapperImpl_right { a1 a2 a3 a4 a5 a6 a7 }   
+                                     ( pubkey : URValue uint256 a1 ) 
+                                     ( wrapper_listing_requests : URValue wrappers_map a2 )
+                                     ( wrapper_code : URValue cell a3 ) 
+                                     ( ext_wallet_code : URValue cell a4 ) 
+                                     ( flex_wallet_code : URValue cell a5 )
+                                     ( workchain_id : URValue int a6 ) 
+                                     ( listing_cfg : URValue ListingConfigLRecord a7 ) 
+                                     : URValue ( address # (wrappers_map ) ) true := 
+ wrapURExpression (ursus_call_with_args (LedgerableWithArgs:= λ7 ) approveWrapperImpl pubkey wrapper_listing_requests wrapper_code ext_wallet_code flex_wallet_code workchain_id listing_cfg ) . 
  
- Notation " 'approveWrapperImpl_' '(' pubkey ',' wrapper_listing_requests ',' wrapper_code ',' ext_wallet_code ',' flex_wallet_code ',' workchain_id ',' listing_cfg ')' " := 
- ( approveWrapperImpl_right 
- pubkey wrapper_listing_requests  wrapper_code  ext_wallet_code  flex_wallet_code  workchain_id  listing_cfg ) 
- (in custom URValue at level 0 , pubkey custom URValue at level 0 
- , wrapper_listing_requests custom URValue at level 0 
- , wrapper_code custom URValue at level 0 
- , ext_wallet_code custom URValue at level 0 
- , flex_wallet_code custom URValue at level 0 
- , workchain_id custom URValue at level 0 
- , listing_cfg custom URValue at level 0 ) : ursus_scope . 
+Notation " 'approveWrapperImpl_' '(' pubkey ',' wrapper_listing_requests ',' wrapper_code ',' ext_wallet_code ',' flex_wallet_code ',' workchain_id ',' listing_cfg ')' " := 
+ ( approveWrapperImpl_right  pubkey wrapper_listing_requests  wrapper_code  ext_wallet_code  flex_wallet_code  workchain_id  listing_cfg ) 
+ (in custom URValue at level 0 , pubkey custom URValue at level 0 , wrapper_listing_requests custom URValue at level 0 
+ , wrapper_code custom URValue at level 0 , ext_wallet_code custom URValue at level 0 , flex_wallet_code custom URValue at level 0 
+ , workchain_id custom URValue at level 0 , listing_cfg custom URValue at level 0 ) : ursus_scope . 
 
-Definition rejectWrapperImpl 
-( pubkey :  uint256 ) 
-( wrapper_listing_requests :  (wrappers_map ) ) 
-( listing_cfg :  ListingConfigLRecord ) 
-: UExpression (wrappers_map ) true . 
-
- 	 	 refine {{ new 'opt_req_info : ( optional WrapperListingRequestLRecord ) @ "opt_req_info" := 
-                   (#{wrapper_listing_requests}) -> extract ( #{pubkey} ) ; { _ } }} . 
- 	 	 refine {{ require_ ( !{ opt_req_info } ,  error_code::wrapper_not_requested  ) ; { _ } }} . 
- 	 	 refine {{ new 'req_info : ( WrapperListingRequestLRecord ) @ "req_info" := 
-                             (!{opt_req_info}) -> get () ; { _ } }} . 
- 	 	 refine {{ new 'remaining_funds : uint128 @ "remaining_funds" := 
-              ( (!{req_info}) ↑ WrapperListingRequest.client_funds ) - 
+Definition rejectWrapperImpl ( pubkey :  uint256 ) ( wrapper_listing_requests : wrappers_map ) 
+                             ( listing_cfg :  ListingConfigLRecord ) : UExpression (wrappers_map ) true . 
+  vararg wrapper_listing_requests "wrapper_listing_requests".
+  refine {{ new 'opt_req_info : optional WrapperListingRequestLRecord @ "opt_req_info" := 
+                   {wrapper_listing_requests} -> extract ( #{pubkey} ) ; { _ } }} . 
+  refine {{ require_ ( ~~!{ opt_req_info } ,  error_code::wrapper_not_requested  ) ; { _ } }} . 
+  refine {{ new 'req_info :  WrapperListingRequestLRecord @ "req_info" := *!{opt_req_info} ; { _ } }} . 
+  refine {{ new 'remaining_funds : uint128 @ "remaining_funds" := 
+              ( !{req_info} ↑ WrapperListingRequest.client_funds ) - 
                 ( (#{listing_cfg}) ↑ ListingConfig.reject_wrapper_cost ) ; { _ } }} . 
-refine {{ IListingAnswerPtr [[  !{req_info} ↑ WrapperListingRequest.client_addr ]]
+  refine {{ IListingAnswerPtr [[  !{req_info} ↑ WrapperListingRequest.client_addr ]]
           with [$ !{remaining_funds} ⇒ { Messsage_ι_value } $]  ⤳ .onWrapperRejected ( #{pubkey} ) ; {_} }}.  
- 	 	 refine {{ return_ (#{wrapper_listing_requests}) }} . 
- Defined .
+  refine {{ return_ !{wrapper_listing_requests} }} . 
+Defined .
  
- Definition rejectWrapperImpl_right { a1 a2 a3 } 
-( pubkey : URValue uint256 a1 ) 
-( wrapper_listing_requests : URValue (wrappers_map ) a2 ) 
-( listing_cfg : URValue ListingConfigLRecord a3 ) 
-: URValue (wrappers_map ) true := 
- wrapURExpression (ursus_call_with_args (LedgerableWithArgs:= λ3 ) rejectWrapperImpl 
- pubkey wrapper_listing_requests listing_cfg ) . 
+ Definition rejectWrapperImpl_right { a1 a2 a3 } ( pubkey : URValue uint256 a1 ) 
+                                    ( wrapper_listing_requests : URValue wrappers_map a2 ) 
+                                    ( listing_cfg : URValue ListingConfigLRecord a3 ) 
+                                    : URValue (wrappers_map ) true := 
+ wrapURExpression (ursus_call_with_args (LedgerableWithArgs:= λ3 ) rejectWrapperImpl  pubkey wrapper_listing_requests listing_cfg ) . 
  
- Notation " 'rejectWrapperImpl_' '(' pubkey , wrapper_listing_requests , listing_cfg ')' " := 
- ( rejectWrapperImpl_right 
- pubkey wrapper_listing_requests listing_cfg ) 
- (in custom URValue at level 0 , pubkey custom URValue at level 0 
- , wrapper_listing_requests custom URValue at level 0 
- , listing_cfg custom URValue at level 0 ) : ursus_scope . 
+Notation " 'rejectWrapperImpl_' '(' pubkey , wrapper_listing_requests , listing_cfg ')' " := 
+ ( rejectWrapperImpl_right pubkey wrapper_listing_requests listing_cfg ) 
+ (in custom URValue at level 0 , pubkey custom URValue at level 0 , 
+  wrapper_listing_requests custom URValue at level 0 , listing_cfg custom URValue at level 0 ) : ursus_scope . 
 
- Definition registerXchgPair 
-( pubkey :  uint256 ) 
-( tip3_major_root : address ) 
-( tip3_minor_root : address ) 
-( min_amount :  uint128 ) 
-( notify_addr : address ) 
-: UExpression address true . 
+Definition registerXchgPair ( pubkey :  uint256 ) ( tip3_major_root : address ) 
+                            ( tip3_minor_root : address ) ( min_amount :  uint128 ) 
+                            ( notify_addr : address ) : UExpression address true . 
 
- refine {{ require_ ( int_value() > (_listing_cfg_ ↑ ListingConfig.register_pair_cost) ,  error_code::not_enough_funds  ) ; { _ } }} . 
- refine {{ require_ ( ~ (  _xchg_pair_listing_requests_ -> contains(#{pubkey}) ) ,  error_code::xchg_pair_with_such_pubkey_already_requested  ) ; { _ } }} . 
- refine {{ _xchg_pair_listing_requests_ -> set_at ( #{pubkey} , 
+  refine {{ require_ ( int_value() > (_listing_cfg_ ↑ ListingConfig.register_pair_cost) ,  error_code::not_enough_funds  ) ; { _ } }} . 
+  refine {{ require_ ( ~  (_xchg_pair_listing_requests_ -> contains ( #{pubkey} )) ,  error_code::xchg_pair_with_such_pubkey_already_requested  ) ; { _ } }} . 
+  refine {{ _xchg_pair_listing_requests_ -> set_at ( #{pubkey} , 
           [ int_sender () , int_value () - _listing_cfg_ ↑ ListingConfig.register_return_value , 
             #{tip3_major_root} , 
             #{tip3_minor_root} , 
             #{min_amount} , 
             #{notify_addr} ] ) ; { _ } }} . 
-       	 	 refine {{ new 'pair_data : ( XchgPairClassTypesModule.DXchgPairLRecord ) @ "pair_data" :=  
+  refine {{ new 'pair_data : ( XchgPairClassTypesModule.DXchgPairLRecord ) @ "pair_data" :=  
                	 	 [$  ( tvm_myaddr () ) ⇒ { DXchgPair_ι_flex_addr_ }  ; 
                       (#{tip3_major_root}) ⇒ { DXchgPair_ι_tip3_major_root_ } ; 
                       (#{tip3_minor_root}) ⇒ { DXchgPair_ι_tip3_minor_root_ } ; 
                       0 ⇒ { DXchgPair_ι_min_amount_ }   ; 
-                     [ # {0%Z} , 0 ]  ⇒ { DXchgPair_ι_notify_addr_ }  
-                   $] ; { _ } }} . 
- 	 	 refine {{ set_int_return_value ( _listing_cfg_ ↑ ListingConfig.register_return_value ) ; { _ } }} . 
- 	 	 refine {{ new ( 'state_init : StateInitLRecord , 'std_addr : uint256 ) @ ( "state_init" , "std_addr" )  := 
-       prepare_xchg_pair_state_init_and_addr_ ( !{pair_data} , _xchg_pair_code_ -> get () ) ; { _ } }} . 
-     (* AL: change workchain_id type *)  
- 	 	 refine {{ return_ [ _workchain_id_  , !{std_addr} ] }} . 
- Defined . 
+                     [ # {0%Z} , 0 ]  ⇒ { DXchgPair_ι_notify_addr_ } $] ; { _ } }} . 
+  refine {{ set_int_return_value ( _listing_cfg_ ↑ ListingConfig.register_return_value ) ; { _ } }} . 
+  refine {{ new ( 'state_init : StateInitLRecord , 'std_addr : uint256 ) 
+              @ ( "state_init" , "std_addr" )  := prepare_xchg_pair_state_init_and_addr_ ( !{pair_data} , _xchg_pair_code_ -> get () ) ; { _ } }} .      
+  refine {{ return_ [ _workchain_id_  , !{std_addr} ] }} . 
+Defined . 
 
- Definition approveXchgPair ( pubkey :  uint256 ) : UExpression address true . 
-  	 	 refine {{ check_owner_ ( ) ; { _ } }} .
- 	 	 refine {{ tvm_accept () ; { _ } }} . 
- 	 	 refine {{ new ( 'xchg_pair : address , 'xchg_pair_listing_requests : xchg_pairs_map  ) @ ( "xchg_pair" , "xchg_pair_listing_requests" ) := 
-               approveXchgPairImpl_ ( #{pubkey} , 
-                                      _xchg_pair_listing_requests_ , 
-                                      _xchg_pair_code_ -> get () , 
-                                      _workchain_id_ , 
-                                      _listing_cfg_ ) ; { _ } }} . 
- 	 	 refine {{ _xchg_pair_listing_requests_ := !{xchg_pair_listing_requests} ; { _ } }} . 
- 	 	 refine {{ if ( #{Internal} ) then { { _ } } else { exit_ {} } ; { _ } }} . 
- 	 	 refine {{ new 'value_gr : uint @ "value_gr" := int_value () ; { _ } }} . 
-  	 refine {{ tvm_rawreserve ( tvm_balance () - !{value_gr} ,  rawreserve_flag::up_to  ) (* ; { _ } *) }} .  
- 	 	 refine {{ set_int_return_flag ( #{SEND_ALL_GAS} ) ; {_} }} .  
- 	 refine {{ return_ !{ xchg_pair } }} . 
- Defined . 
+Definition approveXchgPair ( pubkey :  uint256 ) : UExpression address true . 
+  refine {{ check_owner_ ( ) ; { _ } }} .
+  refine {{ tvm_accept () ; { _ } }} . 
+  refine {{ new ( 'xchg_pair : address , 'xchg_pair_listing_requests : xchg_pairs_map  ) 
+              @ ( "xchg_pair" , "xchg_pair_listing_requests" ) := 
+            approveXchgPairImpl_ ( #{pubkey} , 
+                                  _xchg_pair_listing_requests_ , 
+                                  _xchg_pair_code_ -> get () , 
+                                  _workchain_id_ , 
+                                  _listing_cfg_ ) ; { _ } }} . 
+  refine {{ _xchg_pair_listing_requests_ := !{xchg_pair_listing_requests} ; { _ } }} . 
+  refine {{ { if Internal then _ else {{ return_ {} }} } ; { _ } }} . 
+  refine {{ new 'value_gr : uint @ "value_gr" := int_value () ; { _ } }} . 
+  refine {{ tvm_rawreserve ( tvm_balance () - !{value_gr} ,  rawreserve_flag::up_to  ) ; { _ }  }} .  
+  refine {{ set_int_return_flag ( #{SEND_ALL_GAS} ) }} .  
+  refine {{ return_ !{ xchg_pair } }} . 
+Defined . 
 
-Definition rejectXchgPair ( pubkey : uint256 ) : UExpression XBool true . 
-  	 	 refine {{ check_owner_ ( ) ; { _ } }} .
- 	 	 refine {{ _xchg_pair_listing_requests_ := 
-          rejectXchgPairImpl_ ( #{pubkey} , _xchg_pair_listing_requests_ , _listing_cfg_ ) ; { _ } }} . 
- 	 	 refine {{ if ( #{Internal} ) then { { _ } } else { exit_ {} } ; { _ } }} . 
- 	 	 	 refine {{ new 'value_gr : uint @ "value_gr" := int_value () ; { _ } }} . 
- 	 	 	 refine {{ tvm_rawreserve ( tvm_balance () - !{value_gr} ,  rawreserve_flag::up_to ) (* ; { _ } *) }} .
-  	 	 	 refine {{ set_int_return_flag (  #{SEND_ALL_GAS} ) ; {_} }} .  
- 	 refine {{ return_ TRUE }} . 
- Defined . 
+Definition rejectXchgPair ( pubkey : uint256 ) : UExpression boolean true . 
+  refine {{ check_owner_ ( ) ; { _ } }} .
+  refine {{ _xchg_pair_listing_requests_ := rejectXchgPairImpl_ ( #{pubkey} , _xchg_pair_listing_requests_ , _listing_cfg_ ) ; { _ } }} . 
+  refine {{ { if Internal then _ else {{ return_ {} }} } ; { _ } }} . 
+  refine {{ new 'value_gr : uint @ "value_gr" := int_value () ; { _ } }} . 
+  refine {{ tvm_rawreserve ( tvm_balance () - !{value_gr} ,  rawreserve_flag::up_to ) ; { _ }  }} .
+  refine {{ set_int_return_flag (  #{SEND_ALL_GAS} )  }} .  
+  refine {{ return_ TRUE }} . 
+Defined . 
 
-Definition registerWrapper 
-( pubkey :  uint256 ) 
-( tip3cfg :  ( Tip3ConfigLRecord ) ) 
-: UExpression address true . 
- 	 	 refine {{ require_ ( int_value () 
-           > ( _listing_cfg_ ↑ ListingConfig.register_wrapper_cost ) ,  error_code::not_enough_funds  ) ; { _ } }} . 
- 	 	 refine {{ require_ ( ( ~ (_wrapper_listing_requests_ -> contains ( #{pubkey} ) ) ) ,  error_code::wrapper_with_such_pubkey_already_requested  ) ; { _ } }} . 
- 	 	 refine {{ _wrapper_listing_requests_ -> set_at ( #{pubkey} , 
+Definition registerWrapper ( pubkey :  uint256 ) ( tip3cfg :  Tip3ConfigLRecord ) : UExpression address true . 
+  refine {{ require_ ( int_value () > 
+                        ( _listing_cfg_ ↑ ListingConfig.register_wrapper_cost ) ,  error_code::not_enough_funds  ) ; { _ } }} . 
+  refine {{ require_ ( ( ~ (_wrapper_listing_requests_ -> contains ( #{pubkey} ) ) ) ,  error_code::wrapper_with_such_pubkey_already_requested  ) ; { _ } }} . 
+ 	refine {{ _wrapper_listing_requests_ -> set_at ( #{pubkey} , 
                                [ int_sender () , 
                                  int_value () - _listing_cfg_ ↑ ListingConfig.register_return_value , 
-                                 #{tip3cfg} ] ) ; { _ } }} . 
- 	 	 refine {{ new 'wrapper_data : ( WrapperClassTypesModule.DWrapperLRecord ) @ "wrapper_data" := 
- 	 	 [$ ((#{tip3cfg}) ↑ Tip3Config.name) ⇒ { DWrapper_ι_name_ } ; 
-        ((#{tip3cfg}) ↑ Tip3Config.symbol) ⇒ { DWrapper_ι_symbol_ } ; 
-        ((#{tip3cfg}) ↑ Tip3Config.decimals) ⇒ { DWrapper_ι_decimals_ } ;
+                                 #{tip3cfg} ] ) ; { _ } }} .                            
+  refine {{ new 'wrapper_data :  WrapperClassTypesModule.DWrapperLRecord @ "wrapper_data" := 
+ 	 	 [$ (#{tip3cfg}) ↑ Tip3Config.name ⇒ { DWrapper_ι_name_ } ; 
+        (#{tip3cfg}) ↑ Tip3Config.symbol ⇒ { DWrapper_ι_symbol_ } ; 
+        (#{tip3cfg}) ↑ Tip3Config.decimals ⇒ { DWrapper_ι_decimals_ } ;
         _workchain_id_ ⇒ { DWrapper_ι_workchain_id_ } ;
-          (#{pubkey}) ⇒ { DWrapper_ι_root_public_key_ } ; 
-            (#{pubkey}) ⇒ { DWrapper_ι_root_public_key_ } ;
-           ( tvm_myaddr () ) -> set () ⇒ { DWrapper_ι_owner_address_ } ;
+        (#{pubkey}) ⇒ { DWrapper_ι_root_public_key_ } ; 
+        {} ⇒ { DWrapper_ι_total_granted_ } ;
+        ( tvm_myaddr () ) -> set () ⇒ { DWrapper_ι_owner_address_ } ;
         {} ⇒ { DWrapper_ι_total_granted_ } ; 
         {} ⇒ { DWrapper_ι_internal_wallet_code_ } ; 
-       ( (tvm_myaddr ()) -> set() ) ⇒ { DWrapper_ι_owner_address_ } ;
-       (_listing_cfg_ ↑ ListingConfig.wrapper_keep_balance) ⇒ { DWrapper_ι_start_balance_ } ; 
-        {} ⇒ { DWrapper_ι_external_wallet_ }  
-      $] ; { _ } }} . 
-  	 	 refine {{ set_int_return_value ( _listing_cfg_ ↑  ListingConfig.register_return_value ) ; { _ } }} .  
- 	 	 refine {{ new ( 'wrapper_init :StateInitLRecord , 'wrapper_hash_addr : uint256 ) @ ( "wrapper_init" , "wrapper_hash_addr" ) := 
+        ( tvm_myaddr () ) -> set() ⇒ { DWrapper_ι_owner_address_ } ;
+        (_listing_cfg_ ↑ ListingConfig.wrapper_keep_balance) ⇒ { DWrapper_ι_start_balance_ } ; 
+        {} ⇒ { DWrapper_ι_external_wallet_ }  $] ; { _ } }} . 
+  refine {{ set_int_return_value ( _listing_cfg_ ↑  ListingConfig.register_return_value ) ; { _ } }} .  
+  refine {{ new ( 'wrapper_init :StateInitLRecord , 'wrapper_hash_addr : uint256 ) 
+                  @ ( "wrapper_init" , "wrapper_hash_addr" ) := 
                prepare_wrapper_state_init_and_addr_ ( _wrapper_code_ -> get () , !{wrapper_data} ) ; { _ } }} . 
- 	 	 refine {{ return_  [ _workchain_id_ , !{wrapper_hash_addr} ] }} . 
- Defined . 
+  refine {{ return_  [ _workchain_id_ , !{wrapper_hash_addr} ] }} . 
+Defined . 
  
- Definition approveWrapper ( pubkey :  uint256 ) : UExpression address true . 
-  	 	 refine {{ check_owner_ ( ) ; { _ } }} .
- 	 	 refine {{ tvm_accept () ; { _ } }} . 
- 	 	 refine {{ new ( 'wrapper_addr : address , 
+Definition approveWrapper ( pubkey :  uint256 ) : UExpression address true . 
+  refine {{ check_owner_ ( ) ; { _ } }} .
+  refine {{ tvm_accept () ; { _ } }} . 
+  refine {{ new ( 'wrapper_addr : address , 
                      'new_wrapper_listing_requests : (wrappers_map ) )
                      @ ( "wrapper_addr" , "new_wrapper_listing_requests" ) := 
                  approveWrapperImpl_ ( #{pubkey} , 
@@ -802,28 +806,27 @@ Definition registerWrapper
                                   _flex_wallet_code_ -> get () , 
                                   _workchain_id_ , 
                                   _listing_cfg_ ) ; { _ } }} . 
- 	 	 refine {{ _wrapper_listing_requests_ := !{new_wrapper_listing_requests} ; { _ } }} . 
- 	 	 refine {{ if ( #{Internal} ) then { { _ } } else { exit_ {} } ; { _ } }} . 
- 	 	 refine {{new 'value_gr : uint @ "value_gr" := int_value () ; { _ } }} . 
-  	 refine {{ tvm_rawreserve ( tvm_balance () - !{value_gr} ,  rawreserve_flag::up_to  ) (* ; { _ } *) }} .
-  	 	 	 refine {{ set_int_return_flag ( #{SEND_ALL_GAS} ) ; {_} }} .
- 	 refine {{ return_ !{ wrapper_addr } }} . 
+  refine {{ _wrapper_listing_requests_ := !{new_wrapper_listing_requests} ; { _ } }} . 
+  refine {{ { if Internal then _ else {{ return_ {} }} }; { _ } }} . 
+  refine {{new 'value_gr : uint @ "value_gr" := int_value () ; { _ } }} . 
+  refine {{ tvm_rawreserve ( tvm_balance () - !{value_gr} ,  rawreserve_flag::up_to  )  ; { _ }  }} .
+  refine {{ set_int_return_flag ( #{SEND_ALL_GAS} )  }} .
+  refine {{ return_ !{ wrapper_addr } }} . 
 Defined . 
  
 
- Definition rejectWrapper ( pubkey :  uint256 ) : UExpression XBool true . 
-  	 	 refine {{ check_owner_ ( ) ; { _ } }} .
- 	 	 refine {{ tvm_accept () ; { _ } }} . 
- 	 	 refine {{ _wrapper_listing_requests_ := 
-            rejectWrapperImpl_ ( #{pubkey} , _wrapper_listing_requests_ , _listing_cfg_ ) ; { _ } }} . 
- 	 	 refine {{ if ( #{Internal} ) then { { _ } } else { exit_ {} } ; { _ } }} . 
- 	 	 	 refine {{ new 'value_gr : uint @ "value_gr" := int_value () ; { _ } }} . 
- 	 	 	 refine {{ tvm_rawreserve ( tvm_balance () - !{value_gr} ,  rawreserve_flag::up_to  ) (* ; { _ } *) }} .
-  	 	 	 refine {{ set_int_return_flag ( #{SEND_ALL_GAS} ) ; {_} }} . 
- 	 refine {{ return_ TRUE }} . 
+Definition rejectWrapper ( pubkey :  uint256 ) : UExpression boolean true . 
+  refine {{ check_owner_ ( ) ; { _ } }} .
+  refine {{ tvm_accept () ; { _ } }} . 
+  refine {{ _wrapper_listing_requests_ := rejectWrapperImpl_ ( #{pubkey} , _wrapper_listing_requests_ , _listing_cfg_ ) ; { _ } }} . 
+  refine {{ { if Internal then _ else {{ return_ {} }} }; { _ } }} . 
+  refine {{ new 'value_gr : uint @ "value_gr" := int_value () ; { _ } }} . 
+  refine {{ tvm_rawreserve ( tvm_balance () - !{value_gr} ,  rawreserve_flag::up_to  ) ; { _ } }} .
+  refine {{ set_int_return_flag ( #{SEND_ALL_GAS} ) }} . 
+  refine {{ return_ TRUE }} . 
 Defined . 
 
-Definition isFullyInitialized : UExpression XBool false . 
+Definition isFullyInitialized : UExpression boolean false . 
  	 	 refine {{ return_ ? ( _pair_code_ && 
                          _price_code_ && 
                          _xchg_pair_code_ && 
@@ -831,144 +834,114 @@ Definition isFullyInitialized : UExpression XBool false .
                          _ext_wallet_code_ && 
                          _flex_wallet_code_ && 
                          _wrapper_code_ ) }} . 
- Defined . 
+Defined . 
 
- Definition isFullyInitialized_right  : URValue XBool false := 
- wrapURExpression (ursus_call_with_args (LedgerableWithArgs:= λ0 ) isFullyInitialized 
- ) . 
+Definition isFullyInitialized_right  : URValue boolean false := 
+ wrapURExpression (ursus_call_with_args (LedgerableWithArgs:= λ0 ) isFullyInitialized  ) . 
  
- Notation " 'isFullyInitialized_' '(' ')' " := 
- ( isFullyInitialized_right 
- ) 
+Notation " 'isFullyInitialized_' '(' ')' " :=  ( isFullyInitialized_right ) 
  (in custom URValue at level 0 ) : ursus_scope . 
 
 Definition getTonsCfg : UExpression TonsConfigLRecord false . 
- 	 	 refine {{ return_ _tons_cfg_ }} . 
- Defined .
+  refine {{ return_ _tons_cfg_ }} . 
+Defined .
  
- Definition getTonsCfg_right  : URValue TonsConfigLRecord false := 
- wrapURExpression (ursus_call_with_args (LedgerableWithArgs:= λ0 ) getTonsCfg 
- ) . 
+Definition getTonsCfg_right  : URValue TonsConfigLRecord false := 
+ wrapURExpression (ursus_call_with_args (LedgerableWithArgs:= λ0 ) getTonsCfg  ) . 
  
- Notation " 'getTonsCfg_' '(' ')' " := 
- ( getTonsCfg_right 
- ) 
+Notation " 'getTonsCfg_' '(' ')' " :=  ( getTonsCfg_right ) 
  (in custom URValue at level 0 ) : ursus_scope . 
  
 Definition getListingCfg : UExpression ListingConfigLRecord false . 
- 	 	 refine {{ return_ _listing_cfg_ }} . 
- Defined . 
+  refine {{ return_ _listing_cfg_ }} . 
+Defined . 
  
- Definition getListingCfg_right  : URValue ListingConfigLRecord false := 
- wrapURExpression (ursus_call_with_args (LedgerableWithArgs:= λ0 ) getListingCfg 
- ) . 
+Definition getListingCfg_right  : URValue ListingConfigLRecord false := 
+ wrapURExpression (ursus_call_with_args (LedgerableWithArgs:= λ0 ) getListingCfg ) . 
  
- Notation " 'getListingCfg_' '(' ')' " := 
- ( getListingCfg_right 
- ) 
+Notation " 'getListingCfg_' '(' ')' " :=  ( getListingCfg_right ) 
  (in custom URValue at level 0 ) : ursus_scope . 
  
- Definition getTradingPairCode : UExpression cell true . 
- 	 	 refine {{ return_ ( _pair_code_ -> get () ) }} . 
- Defined . 
+Definition getTradingPairCode : UExpression cell true . 
+  refine {{ return_ ( _pair_code_ -> get () ) }} . 
+Defined . 
  
 Definition getTradingPairCode_right  : URValue cell true := 
- wrapURExpression (ursus_call_with_args (LedgerableWithArgs:= λ0 ) getTradingPairCode 
- ) . 
+ wrapURExpression (ursus_call_with_args (LedgerableWithArgs:= λ0 ) getTradingPairCode ) . 
  
- Notation " 'getTradingPairCode_' '(' ')' " := 
- ( getTradingPairCode_right 
- ) 
+Notation " 'getTradingPairCode_' '(' ')' " := ( getTradingPairCode_right ) 
  (in custom URValue at level 0 ) : ursus_scope . 
  
- Definition getXchgPairCode : UExpression cell true . 
- 	 	 refine {{ return_ ( _xchg_pair_code_ -> get () ) }} . 
- Defined . 
-
- Definition getXchgPairCode_right  : URValue cell true := 
- wrapURExpression (ursus_call_with_args (LedgerableWithArgs:= λ0 ) getXchgPairCode 
- ) . 
- 
- Notation " 'getXchgPairCode_' '(' ')' " := 
- ( getXchgPairCode_right 
- ) 
- (in custom URValue at level 0 ) : ursus_scope . 
-
- Definition getDealsLimit : UExpression uint8 false . 
- 	 	 refine {{ return_ _deals_limit_ }} . 
- Defined . 
-
- Definition getDealsLimit_right  : URValue uint8 false := 
- wrapURExpression (ursus_call_with_args (LedgerableWithArgs:= λ0 ) getDealsLimit 
- ) . 
- 
- Notation " 'getDealsLimit_' '(' ')' " := 
- ( getDealsLimit_right 
- ) 
- (in custom URValue at level 0 ) : ursus_scope . 
-
- Definition getOwnershipInfo : UExpression FlexOwnershipInfoLRecord false . 
- 	 	 refine {{ return_ [ _deployer_pubkey_ , _ownership_description_ , _owner_address_ ] }} . 
- Defined . 
-
- Definition getOwnershipInfo_right  : URValue FlexOwnershipInfoLRecord false := 
- wrapURExpression (ursus_call_with_args (LedgerableWithArgs:= λ0 ) getOwnershipInfo 
- ) . 
- 
- Notation " 'getOwnershipInfo_' '(' ')' " := 
- ( getOwnershipInfo_right 
- ) 
- (in custom URValue at level 0 ) : ursus_scope . 
-
- Definition getWrapperListingRequests : UExpression ( XHMap uint WrapperListingRequestWithPubkeyLRecord ) false . 
- 	 	 refine {{ new 'rv :  ( XHMap uint WrapperListingRequestWithPubkeyLRecord ) @ "rv" := {} ; { _ } }} . 
-     refine {{ for ( 'v : _wrapper_listing_requests_) do { {_ : UEf} } ; { _ } }}. 
-	   refine {{ {rv}  -> push ( [ first ({v}) , second ({v}) ] ) }}.
-  	 refine {{ return_ !{rv} }} . 
+Definition getXchgPairCode : UExpression cell true . 
+  refine {{ return_ ( _xchg_pair_code_ -> get () ) }} . 
 Defined . 
 
- Definition getWrapperListingRequests_right  : URValue ( XHMap uint WrapperListingRequestWithPubkeyLRecord) false := 
- wrapURExpression (ursus_call_with_args (LedgerableWithArgs:= λ0 ) getWrapperListingRequests 
- ) . 
+Definition getXchgPairCode_right  : URValue cell true := 
+ wrapURExpression (ursus_call_with_args (LedgerableWithArgs:= λ0 ) getXchgPairCode ) . 
  
- Notation " 'getWrapperListingRequests_' '(' ')' " := 
- ( getWrapperListingRequests_right 
- ) 
+Notation " 'getXchgPairCode_' '(' ')' " := ( getXchgPairCode_right  ) 
  (in custom URValue at level 0 ) : ursus_scope . 
 
- Definition getTradingPairListingRequests : UExpression ( XHMap uint TradingPairListingRequestWithPubkeyLRecord ) false . 
- 	 	 refine {{ new 'rv :  ( XHMap uint TradingPairListingRequestWithPubkeyLRecord ) @ "rv" := {} ; { _ } }} . 
-     refine {{ for ( 'v : _trading_pair_listing_requests_) do { {_ : UEf} } ; { _ } }}. 
-	   refine {{ {rv}  -> push ( [ first ({v}) , second ({v}) ] ) }}.
- 	 refine {{ return_ !{rv} }} . 
+Definition getDealsLimit : UExpression uint8 false . 
+  refine {{ return_ _deals_limit_ }} . 
 Defined . 
 
- Definition getTradingPairListingRequests_right  : URValue ( XHMap uint TradingPairListingRequestWithPubkeyLRecord ) false := 
- wrapURExpression (ursus_call_with_args (LedgerableWithArgs:= λ0 ) getTradingPairListingRequests 
- ) . 
+Definition getDealsLimit_right  : URValue uint8 false := 
+ wrapURExpression (ursus_call_with_args (LedgerableWithArgs:= λ0 ) getDealsLimit ) . 
  
- Notation " 'getTradingPairListingRequests_' '(' ')' " := 
- ( getTradingPairListingRequests_right 
- ) 
+Notation " 'getDealsLimit_' '(' ')' " := ( getDealsLimit_right ) 
  (in custom URValue at level 0 ) : ursus_scope . 
 
-Definition getXchgPairListingRequests : UExpression ( XHMap uint XchgPairListingRequestWithPubkeyLRecord ) false . 
- 	 	 refine {{ new 'rv :  ( XHMap uint XchgPairListingRequestWithPubkeyLRecord ) @ "rv" := {} ; { _ } }} . 
-     refine {{ for ( 'v : _xchg_pair_listing_requests_) do { {_ : UEf} } ; { _ } }}. 
-	   refine {{ {rv}  -> push ( [ first ({v}) , second ({v}) ] ) }}.
- 	 refine {{ return_ !{rv} }} . 
+Definition getOwnershipInfo : UExpression FlexOwnershipInfoLRecord false . 
+  refine {{ return_ [ _deployer_pubkey_ , _ownership_description_ , _owner_address_ ] }} . 
+Defined . 
+
+Definition getOwnershipInfo_right  : URValue FlexOwnershipInfoLRecord false := 
+ wrapURExpression (ursus_call_with_args (LedgerableWithArgs:= λ0 ) getOwnershipInfo ) . 
+ 
+Notation " 'getOwnershipInfo_' '(' ')' " := ( getOwnershipInfo_right ) 
+ (in custom URValue at level 0 ) : ursus_scope . 
+
+Definition getWrapperListingRequests : UExpression ( mapping uint WrapperListingRequestWithPubkeyLRecord ) false . 
+  refine {{ new 'rv : mapping uint WrapperListingRequestWithPubkeyLRecord @ "rv" := {} ; { _ } }} . 
+  refine {{ for ( 'v : _wrapper_listing_requests_) do { {_ : UEf} } ; { _ } }}. 
+  refine {{ {rv}  -> push ( [ first ( {v} ) , second ( {v} ) ] ) }}.
+  refine {{ return_ !{rv} }} . 
+Defined . 
+
+Definition getWrapperListingRequests_right  : URValue ( mapping uint WrapperListingRequestWithPubkeyLRecord) false := 
+ wrapURExpression (ursus_call_with_args (LedgerableWithArgs:= λ0 ) getWrapperListingRequests ) . 
+ 
+Notation " 'getWrapperListingRequests_' '(' ')' " := ( getWrapperListingRequests_right ) 
+ (in custom URValue at level 0 ) : ursus_scope . 
+
+Definition getTradingPairListingRequests : UExpression ( mapping uint TradingPairListingRequestWithPubkeyLRecord ) false . 
+  refine {{ new 'rv :  mapping uint TradingPairListingRequestWithPubkeyLRecord @ "rv" := {} ; { _ } }} . 
+  refine {{ for ( 'v : _trading_pair_listing_requests_) do { {_ : UEf} } ; { _ } }}. 
+  refine {{ {rv}  -> push ( [ first ( {v} ) , second ( {v} ) ] ) }}.
+  refine {{ return_ !{rv} }} . 
+Defined . 
+
+Definition getTradingPairListingRequests_right  : URValue ( mapping uint TradingPairListingRequestWithPubkeyLRecord ) false := 
+ wrapURExpression (ursus_call_with_args (LedgerableWithArgs:= λ0 ) getTradingPairListingRequests ) . 
+ 
+Notation " 'getTradingPairListingRequests_' '(' ')' " :=  ( getTradingPairListingRequests_right ) 
+ (in custom URValue at level 0 ) : ursus_scope . 
+
+Definition getXchgPairListingRequests : UExpression ( mapping uint XchgPairListingRequestWithPubkeyLRecord ) false . 
+  refine {{ new 'rv :  mapping uint XchgPairListingRequestWithPubkeyLRecord @ "rv" := {} ; { _ } }} . 
+  refine {{ for ( 'v : _xchg_pair_listing_requests_) do { {_ : UEf} } ; { _ } }}. 
+  refine {{ {rv}  -> push ( [ first ( {v} ) , second ( {v} ) ] ) }}.
+  refine {{ return_ !{rv} }} . 
 Defined .
 
- Definition getXchgPairListingRequests_right  : URValue ( XHMap uint XchgPairListingRequestWithPubkeyLRecord ) false := 
- wrapURExpression (ursus_call_with_args (LedgerableWithArgs:= λ0 ) getXchgPairListingRequests 
- ) . 
+Definition getXchgPairListingRequests_right : URValue ( mapping uint XchgPairListingRequestWithPubkeyLRecord ) false := 
+ wrapURExpression (ursus_call_with_args (LedgerableWithArgs:= λ0 ) getXchgPairListingRequests ) . 
  
- Notation " 'getXchgPairListingRequests_' '(' ')' " := 
- ( getXchgPairListingRequests_right 
- ) 
+Notation " 'getXchgPairListingRequests_' '(' ')' " :=  ( getXchgPairListingRequests_right ) 
  (in custom URValue at level 0 ) : ursus_scope . 
 
- Definition getDetails : UExpression FlexDetailsLRecord true .
+Definition getDetails : UExpression FlexDetailsLRecord true .
  	 	 refine {{ return_ [ isFullyInitialized_ ( ) , 
                          getTonsCfg_ ( ) , 
                          getListingCfg_ ( ) , 
@@ -979,90 +952,90 @@ Defined .
                          getWrapperListingRequests_ ( ) , 
                          getTradingPairListingRequests_ ( ) , 
                          getXchgPairListingRequests_ ( ) ] }} . 
- Defined .
+Defined .
 
- Definition getSellPriceCode ( tip3_addr : address ) : UExpression cell true . 
-     refine {{ require_ (FALSE, 0) ; {_} }}.
- 	 	 refine {{ new 'price_code_sl : ( slice ) @ "price_code_sl" := {}
-                          (* _price_code_ -> get () -> to_slice () *) ; { _ } }} . 
- 	 	 (* refine {{ require_ ( (!{price_code_sl}) -> refs () == #{2} ,  error_code::unexpected_refs_count_in_code  ) ; { _ } }} .  *)
- 	 	 refine {{ new 'salt : cell @ "salt" := {} 
-            (*  builder ( ) . stslice ( tvm_myaddr ( ) ) . stslice ( tip3_addr.sl ( ) ) . endc ( ) *) ; { _ } }} . 
- 	 	 refine {{ return_ {} (* builder ( ) . stslice ( !{ price_code_sl } ) . stref ( !{ salt } ) . endc ( ) *) }} . 
- Defined . 
+Notation " x '->' 'sl' '()' " := ( || build (σ {x}) -> endc() -> ctos () || )
+(in custom URValue at level 0 , x custom URValue ) : ursus_scope . 
 
- Definition getXchgPriceCode ( tip3_addr1 : address ) ( tip3_addr2 : address ) : UExpression cell true . 
- 	 	 refine {{ require_ (FALSE, 0) ; {_} }}.
-      refine {{ new 'price_code_sl : ( slice ) @ "price_code_sl" := {}
-               (* _xchg_price_code_ -> get () -> to_slice ()  *) ; { _ } }} . 
- 	 	 (* refine {{ require_ ( (!{price_code_sl}) -> refs () == #{2} ,   error_code::unexpected_refs_count_in_code  ) ; { _ } }} .  *)
- 	 	 refine {{ new 'keys : ( address # address )  @ "keys" := 
-                   [ #{tip3_addr1} , #{tip3_addr2} ] ; { _ } }} . 
- 	 	 refine {{ return_ {} (* builder ( ) . stslice ( !{ price_code_sl } ) . stref ( build ( !{ keys } ) . endc ( ) ) . endc ( ) *) }} . 
- Defined . 
+Definition getSellPriceCode ( tip3_addr : address ) : UExpression cell true .   
+  refine {{ new 'price_code_sl : slice @ "price_code_sl" :=
+                        _price_code_ -> get () -> ctos ()  ; { _ } }} . 
+  refine {{ require_ ( (!{price_code_sl}) -> srefs () == #{2} ,  error_code::unexpected_refs_count_in_code  ) ; { _ } }} .
+  refine {{ new 'salt : cell @ "salt" :=  
+          builder() -> stslice ( tvm_myaddr () -> sl() ) 
+              -> stslice ( (#{tip3_addr}) -> sl () ) -> endc ()  ; { _ } }} . 
+  refine {{ return_ builder () -> stslice ( !{ price_code_sl } ) -> stref ( !{ salt } ) -> endc () }} . 
+Defined . 
 
- Definition getSellTradingPair ( tip3_root : address ) : UExpression address true . 
- 	 	 refine {{ new 'std_addr : uint256 @ "std_addr" := 
-          second (  prepare_trading_pair_ ( ( tvm_myaddr () ) , #{tip3_root} , _pair_code_ -> get () ) ) ; { _ } }} . 
- 	 	 refine {{ return_ [ _workchain_id_ , !{ std_addr } ] }} . 
- Defined . 
+Definition getXchgPriceCode ( tip3_addr1 : address ) 
+                             ( tip3_addr2 : address ) : UExpression cell true . 
+  refine {{ require_ (FALSE, 0) ; {_} }}.
+  refine {{ new 'price_code_sl : slice @ "price_code_sl" := 
+                _xchg_price_code_ -> get () -> ctos ()  ; { _ } }} . 
+ 	refine {{ require_ ( (!{price_code_sl}) -> srefs () == #{2} , error_code::unexpected_refs_count_in_code  ) ; { _ } }} .  
+  refine {{ new 'keys :  address # address   @ "keys" := [ #{tip3_addr1} , #{tip3_addr2} ] ; { _ } }} . 
+  refine {{ return_  builder () -> stslice ( !{ price_code_sl } ) 
+                                -> stref ( build ( σ !{ keys } ) -> endc () ) -> endc ()  }} . 
+Defined . 
+
+Definition getSellTradingPair ( tip3_root : address ) : UExpression address true . 
+  refine {{ new 'std_addr : uint256 @ "std_addr" := 
+      second (  prepare_trading_pair_ ( ( tvm_myaddr () ) , #{tip3_root} , _pair_code_ -> get () ) ) ; { _ } }} . 
+  refine {{ return_ [ _workchain_id_ , !{ std_addr } ] }} . 
+Defined . 
  
- Definition getXchgTradingPair ( tip3_major_root : address ) 
-( tip3_minor_root : address ) : UExpression address true . 
- 	 	 refine {{ new 'myaddr :address @ "myaddr" := ( tvm_myaddr () ) ; { _ } }} . 
- 	 	 refine {{ new 'pair_data : ( XchgPairClassTypesModule.DXchgPairLRecord ) @ "pair_data" :=  
-               	 	 [$            !{ myaddr } ⇒ { DXchgPair_ι_flex_addr_ } ; 
-                        (#{tip3_major_root}) ⇒ { DXchgPair_ι_tip3_major_root_ } ; 
-                        (#{tip3_minor_root}) ⇒ { DXchgPair_ι_tip3_minor_root_ } ; 
-                                          0  ⇒ { DXchgPair_ι_min_amount_ } ; 
-          [#{0%Z} , 0] ⇒ { DXchgPair_ι_notify_addr_ }  
-                   $] ; { _ } }} . 
- 	 	 refine {{ new 'std_addr : uint256 @ "std_addr" := 
+Definition getXchgTradingPair ( tip3_major_root : address )
+                               ( tip3_minor_root : address ) : UExpression address true . 
+  refine {{ new 'myaddr :address @ "myaddr" := ( tvm_myaddr () ) ; { _ } }} . 
+  refine {{ new 'pair_data : ( XchgPairClassTypesModule.DXchgPairLRecord ) @ "pair_data" :=  
+               	 	 [$ !{ myaddr } ⇒ { DXchgPair_ι_flex_addr_ } ; 
+                      (#{tip3_major_root}) ⇒ { DXchgPair_ι_tip3_major_root_ } ; 
+                      (#{tip3_minor_root}) ⇒ { DXchgPair_ι_tip3_minor_root_ } ; 
+                      0  ⇒ { DXchgPair_ι_min_amount_ } ; 
+                      [#{0%Z} , 0] ⇒ { DXchgPair_ι_notify_addr_ } $] ; { _ } }} . 
+  refine {{ new 'std_addr : uint256 @ "std_addr" := 
            second ( prepare_xchg_pair_state_init_and_addr_ ( !{ pair_data } , _xchg_pair_code_ -> get () ) ); { _ } }} . 
- 	 	 refine {{ return_ [ _workchain_id_ , !{ std_addr } ] }} . 
- Defined . 
+  refine {{ return_ [ _workchain_id_ , !{ std_addr } ] }} . 
+Defined . 
 
- 
- Definition _fallback ( msg :  cell ) 
-                      ( msg_body :  ( slice ) ) : UExpression uint false . 
- 	 	 refine {{ return_ 0 }} . 
- Defined . 
+Definition _fallback ( msg : cell ) 
+                     ( msg_body : slice ) : UExpression uint false . 
+  refine {{ return_ 0 }} . 
+Defined . 
 
- Definition prepare_flex_state_init_and_addr ( flex_data :  (ContractLRecord ) ) 
-                                             ( flex_code :  cell ) 
-                    : UExpression ( StateInitLRecord * uint256 ) false . 
- 	 	 refine {{ new 'flex_data_cl : cell @ "flex_data_cl" :=
-              prepare_persistent_data_ ( {} (* flex_replay_protection_t::init ()*) , #{flex_data} ) ; { _ } }} . 
- 	 	 refine {{ new 'flex_init : StateInitLRecord @ "flex_init" := 
+Definition prepare_flex_state_init_and_addr ( flex_data : ContractLRecord ) 
+                                            ( flex_code :  cell ) 
+                    : UExpression ( StateInitLRecord # uint256 ) false . 
+  refine {{ new 'flex_data_cl : cell @ "flex_data_cl" :=
+              prepare_persistent_data_ ( flex_replay_protection_t::init () , #{flex_data} ) ; { _ } }} . 
+  refine {{ new 'flex_init : StateInitLRecord @ "flex_init" := 
              [ {} , {} , (#{flex_code}) -> set () , (!{flex_data_cl}) -> set () , {} ] ; { _ } }} . 
- 	 	 refine {{ new 'flex_init_cl : cell @ "flex_init_cl" := 
+  refine {{ new 'flex_init_cl : cell @ "flex_init_cl" := 
                        build ( σ !{ flex_init } ) -> make_cell () ; { _ } }} . 
- 	 	 refine {{ return_ [ !{ flex_init } , tvm_hash ( !{flex_init_cl} )  ] }} . 
- Defined . 
+  refine {{ return_ [ !{ flex_init } , tvm_hash ( !{flex_init_cl} )  ] }} . 
+Defined . 
 
  
- Definition prepare_internal_wallet_state_init_and_addr 
-( name :  ( XString ) ) 
-( symbol :  ( XString ) )
- ( decimals :  uint8 )
- ( root_public_key :  uint256 )
- ( wallet_public_key :  uint256 ) 
-( root_address : address ) 
-( owner_address :  ( optional address ) ) 
-( code :  cell ) 
-( workchain_id :  int ) 
-: UExpression ( StateInitLRecord * uint256 ) false . 
- 	 	 refine {{ new 'wallet_data : ( TONTokenWalletClassTypesModule.DTONTokenWalletInternalLRecord ) @ "wallet_data" := 
-                 [ #{name} , #{symbol} , #{decimals} , 0 , #{root_public_key} , 
-                   #{wallet_public_key} , #{root_address} , #{owner_address} , 
-                   {} , #{code} , #{workchain_id} ] ; { _ } }} . 
- 	 	 refine {{ new 'wallet_data_cl : cell @ "wallet_data_cl" := 
-               prepare_persistent_data_ ( {} , !{wallet_data} ) ; { _ } }} . 
- 	 	 refine {{ new 'wallet_init : StateInitLRecord @ "wallet_init" := 
-              [ {} , {} , (#{code}) -> set () , (!{wallet_data_cl}) -> set () , {} ] ; { _ } }} . 
- 	 	 refine {{ new 'wallet_init_cl : cell @ "wallet_init_cl" := 
-                      build ( σ !{ wallet_init } ) -> make_cell () ; { _ } }} . 
- 	 	 refine {{ return_ [ !{ wallet_init } ,  tvm_hash ( !{wallet_init_cl} )  ] }} . 
+Definition prepare_internal_wallet_state_init_and_addr ( name :  String ) 
+                                                        ( symbol :  String )
+                                                        ( decimals :  uint8 )
+                                                        ( root_public_key :  uint256 )
+                                                        ( wallet_public_key :  uint256 ) 
+                                                        ( root_address : address ) 
+                                                        ( owner_address : optional address ) 
+                                                        ( code :  cell ) 
+                                                        ( workchain_id : int ) : UExpression ( StateInitLRecord * uint256 ) false . 
+  refine {{ new 'wallet_data : ( TONTokenWalletClassTypesModule.DTONTokenWalletInternalLRecord ) @ "wallet_data" := 
+              [ #{name} , #{symbol} , #{decimals} , 0 , #{root_public_key} , 
+                #{wallet_public_key} , #{root_address} , #{owner_address} , 
+                {} , #{code} , #{workchain_id} ] ; { _ } }} . 
+  refine {{ new 'wallet_data_cl : cell @ "wallet_data_cl" := 
+            prepare_persistent_data_ ( {} , !{wallet_data} ) ; { _ } }} . 
+  refine {{ new 'wallet_init : StateInitLRecord @ "wallet_init" := 
+          [ {} , {} , (#{code}) -> set () , (!{wallet_data_cl}) -> set () , {} ] ; { _ } }} . 
+  refine {{ new 'wallet_init_cl : cell @ "wallet_init_cl" := 
+                  build ( σ !{ wallet_init } ) -> make_cell () ; { _ } }} . 
+  refine {{ return_ [ !{ wallet_init } ,  tvm_hash ( !{wallet_init_cl} )  ] }} . 
 Defined . 
 
 End FuncsInternal.
